@prefix steam: <https://wikipunk.net/steam/> .
@prefix owl: <http://www.w3.org/2002/07/owl#> .
@prefix rdf: <http://www.w3.org/1999/02/22-rdf-syntax-ns#> .
@prefix rdfs: <http://www.w3.org/2000/01/rdf-schema#> .
@prefix xsd: <http://www.w3.org/2001/XMLSchema#> .
@prefix schema: <http://schema.org/> .

steam: a owl:Ontology ;
  rdfs:label "Steam Ontology" ;
  rdfs:comment  "A work-in-progress ontology describing the Steam platform. Use the rdfs:label property on tag classes to get the name of the tag as catalogued by Steam." ;
  rdfs:seeAlso <https://partner.steamgames.com/doc/home>, <https://partner.steamgames.com/doc/store/tags> .

steam:Tag a owl:Class ;
  rdfs:subClassOf schema:Thing ;
  rdfs:label "Tag" ;
  rdfs:comment "A tag used to categorize a game on Steam" .

# Tag classes

steam:TopLevelGenre a owl:Class ;
  rdfs:subClassOf steam:Tag ;
  rdfs:label "Top Level Genre" ;
  rdfs:comment "A top level genre used to categorize a game on Steam" .

steam:Genre a owl:Class ;
  rdfs:subClassOf steam:Tag ;
  rdfs:label "Genre" ;
  rdfs:comment "A genre used to categorize a game on Steam" .

steam:SubGenre a owl:Class ;
  rdfs:subClassOf steam:Tag ;
  rdfs:label "Sub-Genre" ;
  rdfs:comment "A sub-genre used to categorize a game on Steam" .

steam:VisualsAndViewpoint a owl:Class ;
  rdfs:subClassOf steam:Tag ;
  rdfs:label "Visuals and Viewpoint" ;
  rdfs:comment "A tag used to describe the visuals and viewpoint of a game on Steam" .

steam:ThemesAndMoods a owl:Class ;
  rdfs:subClassOf steam:Tag ;
  rdfs:label "Themes and Moods" ;
  rdfs:comment "A tag used to describe the themes and moods of a game on Steam" .

steam:Features a owl:Class ;
  rdfs:subClassOf steam:Tag ;
  rdfs:label "Features" ;
  rdfs:comment "A tag used to describe the features of a game on Steam" .

steam:Players a owl:Class, schema:GamePlayMode ;
  rdfs:subClassOf steam:Tag ;
  rdfs:label "Players" ;
  rdfs:comment "A tag used to describe the player options of a game on Steam" .

steam:Other a owl:Class ;
  rdfs:subClassOf steam:Tag ;
  rdfs:label "Other" ;
  rdfs:comment "A tag used to categorize other aspects of a game on Steam" .

steam:Software a owl:Class ;
  rdfs:subClassOf steam:Tag ;
  rdfs:label "Software" ;
  rdfs:comment "A tag used to categorize the software of a game on Steam" .

steam:Assessments a owl:Class ;
  rdfs:subClassOf steam:Tag ;
  rdfs:label "Assessments" ;
  rdfs:comment "A tag used to categorize the assessments of a game on Steam" .

steam:Ratings a owl:Class ;
  rdfs:subClassOf steam:Tag ;
  rdfs:label "Ratings" ;
  rdfs:comment "A tag used to categorize the ratings of a game on Steam" .

steam:HardwareInput a owl:Class ;
  rdfs:subClassOf steam:Tag ;
  rdfs:label "Hardware Input" ;
  rdfs:comment "A tag used to categorize the hardware input of a game on Steam" .

steam:Funding a owl:Class ;
  rdfs:subClassOf steam:Tag ;
  rdfs:label "Funding" ;
  rdfs:comment "A tag used to categorize the funding of a game on Steam" .

# Top Level Genre tags

steam:Action a owl:Class, steam:TopLevelGenre ;
  rdfs:label "Action" ;
  rdfs:comment "Action games emphasize physical challenges that require hand-eye coordination and motor skill to overcome. They center around the player controlling a character in a world where they must navigate obstacles and fight enemies to succeed." ;
  rdfs:seeAlso <http://dbpedia.org/resource/Action_game> ;
  schema:url <https://store.steampowered.com/tags/en/Action/> .

steam:Adventure a owl:Class, steam:TopLevelGenre ;
  rdfs:label "Adventure" ;
  rdfs:comment "Adventure games focus on puzzle solving within a narrative framework, generally with few or no action elements. These games encourage players to explore, interact with different objects, and solve complex puzzles to progress the story." ;
  rdfs:seeAlso <http://dbpedia.org/resource/Adventure_game> ;
  schema:url <https://store.steampowered.com/tags/en/Adventure/> .

steam:Casual a owl:Class, steam:TopLevelGenre ;
  rdfs:label "Casual" ;
  rdfs:comment "Casual games are designed to be easily picked up and put down again, allowing for potentially short bursts of play. They often have simpler rules, shorter sessions, and less learned skill than hardcore games." ;
  rdfs:seeAlso <http://dbpedia.org/resource/Casual_game> ;
  schema:url <https://store.steampowered.com/tags/en/Casual/> .

steam:Experimental a owl:Class, steam:TopLevelGenre, steam:Genre ;
  rdfs:label "Experimental" ;
  rdfs:comment "Experimental games are those that challenge the status quo of gaming and offer a unique, sometimes strange, gaming experience. These games often explore new game mechanics, storytelling methods, and art styles." ;
  rdfs:seeAlso <http://dbpedia.org/resource/Art_game> ;
  schema:url <https://store.steampowered.com/tags/en/Experimental/> .

steam:Puzzle a owl:Class, steam:TopLevelGenre ;
  rdfs:label "Puzzle" ;
  rdfs:comment "Puzzle games focus on problem solving and logical thinking. They challenge the player to solve head-scratching puzzles and often offer a slower paced, more relaxing gaming experience." ;
  rdfs:seeAlso <http://dbpedia.org/resource/Puzzle_video_game> ;
  schema:url <https://store.steampowered.com/tags/en/Puzzle/> .

steam:Racing a owl:Class, steam:TopLevelGenre ;
  rdfs:label "Racing" ;
  rdfs:comment "Racing games simulate the competition of racing, where the player controls a vehicle or other transport. They often have a time limit, and can include obstacles and competitors to beat." ;
  rdfs:seeAlso <http://dbpedia.org/resource/Racing_video_game> ;
  schema:url <https://store.steampowered.com/tags/en/Racing/> .

steam:RPG a owl:Class, steam:TopLevelGenre ;
  rdfs:label "RPG" ;
  rdfs:comment "Role-playing games (RPGs) often involve story-telling and narrative elements, character development, complexity, as well as replayability and immersion. The player controls a character in a world where they undertake quests and challenges." ;
  rdfs:seeAlso <http://dbpedia.org/resource/Role-playing_video_game> ;
  schema:url <https://store.steampowered.com/tags/en/RPG/> .

steam:Simulation a owl:Class, steam:TopLevelGenre ;
  rdfs:label "Simulation" ;
  rdfs:comment "Simulation games are designed to accurately simulate real-world activities. They can cover a variety of activities, including driving vehicles, managing a business, or living a life." ;
  rdfs:seeAlso <http://dbpedia.org/resource/Simulation_video_game> ;
  schema:url <https://store.steampowered.com/tags/en/Simulation/> .

steam:Sports a owl:Class, steam:TopLevelGenre ;
  rdfs:label "Sports" ;
  rdfs:comment "Sports games simulate the practice of traditional physical sports. This can be team sports such as soccer, basketball, or individual activities like golf, fishing, skateboarding." ;
  rdfs:seeAlso <http://dbpedia.org/resource/Sports_game> ;
  schema:url <https://store.steampowered.com/tags/en/Sports/> .

steam:Strategy a owl:Class, steam:TopLevelGenre ;
  rdfs:label "Strategy" ;
  rdfs:comment "Strategy games require strategic, tactical, and sometimes logistical challenges. Many games also offer economic challenges and exploration." ;
  rdfs:seeAlso <http://dbpedia.org/resource/Strategy_video_game> ;
  schema:url <https://store.steampowered.com/tags/en/Strategy/> .

steam:Tabletop a owl:Class, steam:TopLevelGenre ;
  rdfs:label "Tabletop" ;
  rdfs:comment "Tabletop games are those that are normally played on a table or other flat surface, such as board games, card games, dice games, miniatures wargames, tile-based games and role-playing games. In the digital context, these games are often adaptations of traditional tabletop games." ;
  rdfs:seeAlso <http://dbpedia.org/resource/Tabletop_game> ;
  schema:url <https://store.steampowered.com/tags/en/Tabletop/> .

# Genre tags

steam:ActionRPG a owl:Class, steam:Genre ;
  rdfs:label "Action RPG" ;
  rdfs:comment "Action RPG games combine elements of action games with elements of role-playing games, typically featuring real-time combat where the player has direct control over characters, as opposed to turn-based or menu-based combat." ;
  rdfs:seeAlso <http://dbpedia.org/resource/Action_role-playing_game> ;
  schema:url <https://store.steampowered.com/tags/en/Action%20RPG/> .

steam:ActionAdventure a owl:Class, steam:Genre ;
  rdfs:label "Action-Adventure" ;
  rdfs:comment "Action-Adventure games blend elements of action games with elements of adventure games, typically featuring an emphasis on combat along with puzzle-solving and item-gathering." ;
  rdfs:seeAlso <http://dbpedia.org/resource/Action-adventure_game> ;
  schema:url <https://store.steampowered.com/tags/en/Action-Adventure/> .

steam:Arcade a owl:Class, steam:Genre ;
  rdfs:label "Arcade" ;
  rdfs:comment "Arcade games are focused on short, simple gameplay offering immediate satisfaction but also challenge and replayability. They often mimic games found in real-world arcades, like racing, shooting, or sports games." ;
  rdfs:seeAlso <http://dbpedia.org/resource/Arcade_game> ;
  schema:url <https://store.steampowered.com/tags/en/Arcade/> .

steam:AutoBattler a owl:Class, steam:Genre ;
  rdfs:label "Auto Battler" ;
  rdfs:comment "Auto Battler games, also known as auto chess, involve automatic battles between characters controlled by the game rather than the player. Players typically focus on strategy, such as character placement and upgrades." ;
  schema:url <https://store.steampowered.com/tags/en/Auto%20Battler/> .

steam:AutomobileSim a owl:Class, steam:Genre ;
  rdfs:label "Automobile Sim" ;
  rdfs:comment "Automobile Sim games simulate the experience of driving or racing cars. They often focus on realistic physics and vehicle handling, as well as potentially managing aspects of the car's performance such as fuel usage or mechanical wear." ;
  rdfs:subClassOf steam:Simulation, steam:Racing ;
  schema:url <https://store.steampowered.com/tags/en/Automobile%20Sim/> .

steam:BaseBuilding a owl:Class, steam:Genre ;
  rdfs:label "Base Building" ;
  rdfs:comment "Base Building games focus on the construction and management of a home base or headquarters for the player. This often involves gathering resources, managing infrastructure, and defending against attacks." ;
  schema:url <https://store.steampowered.com/tags/en/Base%20Building/> .

steam:Baseball a owl:Class, steam:Genre ;
  rdfs:label "Baseball" ;
  rdfs:comment "Baseball games simulate the sport of baseball, allowing players to control a team and compete in games or seasons. They often focus on realistic gameplay and statistics." ;
  rdfs:subClassOf steam:Sports ;
  rdfs:seeAlso <http://dbpedia.org/resource/Baseball> ;
  schema:url <https://store.steampowered.com/tags/en/Baseball/> .

steam:Basketball a owl:Class, steam:Genre ;
  rdfs:label "Basketball" ;
  rdfs:comment "Basketball games simulate the sport of basketball, allowing players to control a team and compete in games or seasons. They often focus on realistic gameplay and statistics." ;
  rdfs:subClassOf steam:Sports ;
  rdfs:seeAlso <http://dbpedia.org/resource/Basketball> ;
  schema:url <https://store.steampowered.com/tags/en/Basketball/> .

steam:BattleRoyale a owl:Class, steam:Genre ;
  rdfs:label "Battle Royale" ;
  rdfs:comment "Battle Royale games involve numerous players that compete to be the last person or team standing. These games often involve a shrinking play area to bring players closer together over time." ;
  rdfs:subClassOf [
    a owl:Restriction ;
    owl:onProperty schema:playMode ;
    owl:hasValue schema:MultiPlayer
    ] ;
  rdfs:seeAlso <http://dbpedia.org/resource/Battle_royale_game> ;
  schema:url <https://store.steampowered.com/tags/en/Battle%20Royale/> .

steam:BMX a owl:Class, steam:Genre ;
  rdfs:label "BMX" ;
  rdfs:comment "BMX games simulate the sport of BMX biking, allowing players to perform tricks, compete in races, or explore environments on a BMX bike." ;
  rdfs:subClassOf steam:Sports, steam:Racing ;
  rdfs:seeAlso <http://dbpedia.org/resource/BMX> ;
  schema:url <https://store.steampowered.com/tags/en/BMX/> .

steam:BoardGame a owl:Class, steam:Genre ;
  rdfs:label "Board Game" ;
  rdfs:comment "Board Game genre includes games that are digital adaptations of traditional or modern board games. They often involve strategic decision making, and can be played solo or multiplayer." ;
  rdfs:subClassOf steam:Tabletop ;
  rdfs:seeAlso <http://dbpedia.org/resource/Board_game> ;
  schema:url <https://store.steampowered.com/tags/en/Board%20Game/> .

steam:Bowling a owl:Class, steam:Genre ;
  rdfs:label "Bowling" ;
  rdfs:comment "Bowling games simulate the sport of bowling, allowing players to compete in games or tournaments. They often focus on realistic physics and gameplay." ;
  rdfs:subClassOf steam:Sports ;
  rdfs:seeAlso <http://dbpedia.org/resource/Bowling> ;
  schema:url <https://store.steampowered.com/tags/en/Bowling/> .

steam:Building a owl:Class, steam:Genre ;
  rdfs:label "Building" ;
  rdfs:comment "Building games focus on the construction of structures or environments. They often involve gathering resources, planning and designing buildings, and managing infrastructure." ;
  rdfs:subClassOf steam:Simulation ;
  rdfs:seeAlso <http://dbpedia.org/resource/Construction_and_management_simulation> ;
  schema:url <https://store.steampowered.com/tags/en/Building/> .

steam:CardGame a owl:Class, steam:Genre ;
  rdfs:label "Card Game" ;
  rdfs:comment "Card games are digital adaptations of traditional or modern card games. They often involve strategic decision making, and can be played solo or multiplayer." ;
  rdfs:subClassOf steam:Tabletop ;
  rdfs:seeAlso <http://dbpedia.org/resource/Card_game> ;
  schema:url <https://store.steampowered.com/tags/en/Card%20Game/> .

steam:CharacterActionGame a owl:Class, steam:Genre ;
  rdfs:label "Character Action Game" ;
  rdfs:comment "Character Action Games are action games that allow players to control a single, or sometimes multiple, characters. These games often feature combat and exploration." ;
  rdfs:subClassOf steam:Action ;
  schema:url <https://store.steampowered.com/tags/en/Character%20Action%20Game/> .

steam:Chess a owl:Class, steam:Genre ;
  rdfs:label "Chess" ;
  rdfs:comment "Chess games are digital adaptations of the traditional board game of chess. They often allow for play against AI or human opponents, and may offer additional features like tutorials or puzzles." ;
  rdfs:subClassOf steam:BoardGame ;
  rdfs:seeAlso <http://dbpedia.org/resource/Chess> ;
  schema:url <https://store.steampowered.com/tags/en/Chess/> .

steam:Clicker a owl:Class, steam:Genre ;
  rdfs:label "Clicker" ;
  rdfs:comment "Clicker games, also known as incremental or idle games, involve simple gameplay that can often run without player intervention. They often involve clicking or tapping to gain some form of currency, which can be used to purchase upgrades." ;
  rdfs:subClassOf steam:Casual ;  
  rdfs:seeAlso <http://dbpedia.org/resource/Incremental_game> ;
  schema:sameAs steam:Idler ;  
  schema:url <https://store.steampowered.com/tags/en/Clicker/> .

steam:Cycling a owl:Class, steam:Genre ;
  rdfs:label "Cycling" ;
  rdfs:comment "Cycling games simulate the sport of cycling, allowing players to compete in races or explore environments on a bike." ;
  rdfs:subClassOf steam:Sports, steam:Racing ;
  schema:url <https://store.steampowered.com/tags/en/Cycling/> .

steam:Diplomacy a owl:Class, steam:Genre ;
  rdfs:label "Diplomacy" ;
  rdfs:comment "Diplomacy games involve negotiation, strategy, and social interaction. Players often need to form alliances, make deals, or negotiate with other players to achieve their goals." ;
  rdfs:subClassOf steam:Strategy ;
  schema:url <https://store.steampowered.com/tags/en/Diplomacy/> .

steam:Esports a owl:Class, steam:Genre ;
  rdfs:label "eSports" ;
  rdfs:comment "Esports games are competitive games that are often played in professional competitions. They often require high levels of skill and strategy, and have large online communities." ;
  rdfs:seeAlso <http://dbpedia.org/resource/Esports> ;
  rdfs:subClassOf steam:Sports ;
  schema:url <https://store.steampowered.com/tags/en/eSports/> .

steam:Exploration a owl:Class, steam:Genre ;
  rdfs:label "Exploration" ;
  rdfs:comment "Exploration games focus on the act of exploring an environment. They often feature open-world settings, and encourage players to explore and discover new areas, items, or storylines." ;
  schema:url <https://store.steampowered.com/tags/en/Exploration/> .

steam:FarmingSim a owl:Class, steam:Genre ;
  rdfs:label "Farming Sim" ;
  rdfs:comment "Farming Sim games simulate the experience of farming, including the cultivation of crops, raising of livestock, and management of a farm. They often involve elements of strategy and resource management." ;
  rdfs:subClassOf steam:Simulation ;
  schema:url <https://store.steampowered.com/tags/en/Farming%20Sim/> .

steam:Fighting a owl:Class, steam:Genre ;
  rdfs:label "Fighting" ;
  rdfs:comment "Fighting games are characterized by close combat between two fighters or groups of fighters, often set in arenas. Players must master techniques, combos, and strategy to overcome their opponents." ;
  rdfs:subClassOf steam:Action ;
  rdfs:seeAlso <http://dbpedia.org/resource/Fighting_game> ;
  schema:url <https://store.steampowered.com/tags/en/Fighting/> .

steam:Football a owl:Class, steam:Genre ;
  rdfs:label "Football" ;
  rdfs:comment "Football games simulate the sport of football, allowing players to control a team and compete in matches or seasons. They often focus on realistic gameplay and statistics." ;
  rdfs:subClassOf steam:Sports ;
  rdfs:seeAlso <http://dbpedia.org/resource/Football_game> ;
  schema:url <https://store.steampowered.com/tags/en/Football/> .

steam:GodGame a owl:Class, steam:Genre ;
  rdfs:label "God Game" ;
  rdfs:comment "God games are a type of game where players control a character with divine powers. They often involve elements of creation, terraforming, and control over nature." ;
  rdfs:subClassOf steam:Simulation ;
  rdfs:seeAlso <http://dbpedia.org/resource/God_game> ;
  schema:url <https://store.steampowered.com/tags/en/God%20Game/> .

steam:Golf a owl:Class, steam:Genre ;
  rdfs:label "Golf" ;
  rdfs:comment "Golf games simulate the sport of golf, allowing players to compete in matches or tournaments. They often focus on realistic physics and gameplay." ;
  rdfs:seeAlso <http://dbpedia.org/resource/Golf_game> ;
  rdfs:subClassOf steam:Sports ;
  schema:url <https://store.steampowered.com/tags/en/Golf/> .

steam:Hacking a owl:Class, steam:Genre ;
  rdfs:label "Hacking" ;
  rdfs:comment "Hacking games involve elements of computer hacking. They often require players to solve puzzles, exploit systems, or engage in simulated computer hacking tasks." ;
  schema:url <https://store.steampowered.com/tags/en/Hacking/> .

steam:HiddenObject a owl:Class, steam:Genre ;
  rdfs:label "Hidden Object" ;
  rdfs:comment "Hidden Object games require players to find specific items from a list that are hidden within a picture or scene." ;
  rdfs:subClassOf steam:Puzzle ;
  rdfs:seeAlso <http://dbpedia.org/resource/Hidden_object_game> ;
  schema:url <https://store.steampowered.com/tags/en/Hidden%20Object/> .

steam:Hockey a owl:Class, steam:Genre ;
  rdfs:label "Hockey" ;
  rdfs:comment "Hockey games simulate the sport of hockey, allowing players to control a team and compete in matches or seasons. They often focus on realistic gameplay and statistics." ;
  rdfs:subClassOf steam:Sports ;
  schema:url <https://store.steampowered.com/tags/en/Hockey/> .

steam:Idler a owl:Class, steam:Genre ;
  rdfs:label "Idler" ;
  rdfs:comment "Idler games, also known as incremental or idle games, involve simple gameplay that can often run without player intervention. They often involve clicking or tapping to gain some form of currency, which can be used to purchase upgrades." ;
  rdfs:subClassOf steam:Casual ;
  rdfs:seeAlso <http://dbpedia.org/resource/Incremental_game> ;
  schema:sameAs steam:Clicker ;
  schema:url <https://store.steampowered.com/tags/en/Idler/> .

steam:InteractiveFiction a owl:Class, steam:Genre ;
  rdfs:label "Interactive Fiction" ;
  rdfs:comment "Interactive Fiction games are games that emphasize narrative and player choice. They often involve complex branching narratives and multiple endings." ;
  rdfs:seeAlso <http://dbpedia.org/resource/Interactive_fiction> ;
  schema:url <https://store.steampowered.com/tags/en/Interactive%20Fiction/> .

steam:Management a owl:Class, steam:Genre ;
  rdfs:label "Management" ;
  rdfs:comment "Management games involve managing resources and making strategic decisions. They often require players to manage businesses, cities, or other entities." ;
  rdfs:subClassOf steam:Simulation ;
  rdfs:seeAlso <http://dbpedia.org/resource/Construction_and_management_simulation> ;
  schema:url <https://store.steampowered.com/tags/en/Management/> .

steam:Match3 a owl:Class, steam:Genre ;
  rdfs:label "Match 3" ;
  rdfs:comment "Match 3 games require players to match three or more items of the same type to achieve a goal. They often involve puzzle-solving and strategic thinking." ;
  rdfs:subClassOf steam:Puzzle ;
  rdfs:seeAlso <http://dbpedia.org/resource/Tile-matching_video_game> ;
  schema:url <https://store.steampowered.com/tags/en/Match%203/> .

steam:MedicalSim a owl:Class, steam:Genre ;
  rdfs:label "Medical Sim" ;
  rdfs:comment "Medical Sim games simulate medical scenarios or procedures. They often require players to diagnose and treat patients, manage a medical facility, or perform simulated surgeries." ;
  rdfs:subClassOf steam:Simulation ;
  rdfs:seeAlso <http://dbpedia.org/resource/Medical_simulation> ;
  schema:url <https://store.steampowered.com/tags/en/Medical%20Sim/> .

steam:MiniGolf a owl:Class, steam:Genre ;
  rdfs:label "Mini Golf" ;
  rdfs:comment "Mini Golf games simulate the sport of mini golf, allowing players to compete in matches or tournaments. They often focus on realistic physics and gameplay." ;
  rdfs:subClassOf steam:Sports ;
  rdfs:seeAlso <http://dbpedia.org/resource/Miniature_golf> ;
  schema:url <https://store.steampowered.com/tags/en/Mini%20Golf/> .

steam:Mining a owl:Class, steam:Genre ;
  rdfs:label "Mining" ;
  rdfs:comment "Mining games involve the extraction of valuable minerals or other geological materials from the earth. They often require players to manage resources, explore environments, and develop mining operations." ;
  schema:url <https://store.steampowered.com/tags/en/Mining/> .

steam:MMORPG a owl:Class, steam:Genre ;
  rdfs:label "MMORPG" ;
  rdfs:comment "MMORPGs (Massively Multiplayer Online Role-Playing Games) are games that involve large numbers of players interacting in a virtual world. They often involve character development, quests, and multiplayer cooperation or competition." ;
  rdfs:subClassOf steam:RPG ;
  rdfs:subClassOf [
    a owl:Restriction ;
    owl:onProperty schema:playMode ;
    owl:hasValue schema:MultiPlayer
    ] ;
  rdfs:seeAlso <http://dbpedia.org/resource/Massively_multiplayer_online_role-playing_game> ;
  schema:url <https://store.steampowered.com/tags/en/MMORPG/> .

steam:MOBA a owl:Class, steam:Genre ;
  rdfs:label "MOBA" ;
  rdfs:comment "MOBA (Multiplayer Online Battle Arena) games involve teams of players competing against each other in an arena. They often require strategic decision-making, teamwork, and player skill." ;
  rdfs:subClassOf steam:Strategy ;
  rdfs:subClassOf [
    a owl:Restriction ;
    owl:onProperty schema:playMode ;
    owl:hasValue schema:MultiPlayer
    ] ;
  rdfs:seeAlso <http://dbpedia.org/resource/Multiplayer_online_battle_arena> ;
  schema:url <https://store.steampowered.com/tags/en/MOBA/> .

steam:Motocross a owl:Class, steam:Genre ;
  rdfs:label "Motocross" ;
  rdfs:comment "Motocross games simulate the sport of motocross, allowing players to compete in races or perform stunts on a motocross bike." ;
  rdfs:subClassOf steam:Racing, steam:Sports ;
  rdfs:seeAlso <http://dbpedia.org/resource/Motocross_video_game> ;
  schema:url <https://store.steampowered.com/tags/en/Motocross/> .

steam:OpenWorld a owl:Class, steam:Genre ;
  rdfs:label "Open World" ;
  rdfs:comment "Open World games provide a large, open environment for players to explore and interact with. They often allow players to choose their own objectives and play at their own pace." ;
  rdfs:seeAlso <http://dbpedia.org/resource/Open_world> ;
  schema:url <https://store.steampowered.com/tags/en/Open%20World/> .

steam:OutbreakSim a owl:Class, steam:Genre ;
  rdfs:label "Outbreak Sim" ;
  rdfs:comment "Outbreak Sim games simulate the spread of diseases or other outbreaks and often involve strategy and management elements." ;
  rdfs:subClassOf steam:Simulation ;
  schema:url <https://store.steampowered.com/tags/en/Outbreak%20Sim/> .

steam:PartyBasedRPG a owl:Class, steam:Genre ;
  rdfs:label "Party-Based RPG" ;
  rdfs:comment "Party-Based RPGs are role-playing games where players control a group of characters, often with different abilities and roles, and must use teamwork and strategy to succeed." ;
  rdfs:subClassOf steam:RPG ;
  schema:url <https://store.steampowered.com/tags/en/Party-Based%20RPG/> .

steam:Pinball a owl:Class, steam:Genre ;
  rdfs:label "Pinball" ;
  rdfs:comment "Pinball games simulate the classic arcade game of pinball, where players use flippers to hit a ball and score points." ;
  rdfs:subClassOf steam:Arcade ;
  rdfs:seeAlso <http://dbpedia.org/resource/Pinball> ;
  schema:url <https://store.steampowered.com/tags/en/Pinball/> .

steam:Platformer a owl:Class, steam:Genre ;
  rdfs:label "Platformer" ;
  rdfs:comment "Platformer games involve guiding a character through levels and overcoming obstacles, often by jumping onto platforms at different heights." ;
  rdfs:seeAlso <http://dbpedia.org/resource/Platform_game> ;
  schema:url <https://store.steampowered.com/tags/en/Platformer/> .

steam:PointAndClick a owl:Class, steam:Genre ;
  rdfs:label "Point & Click" ;
  rdfs:comment "Point & Click games involve interacting with the environment and solving puzzles through a point-and-click interface." ;
  schema:url <https://store.steampowered.com/tags/en/Point%20&%20Click/> .

steam:Rhythm a owl:Class, steam:Genre ;
  rdfs:label "Rhythm" ;
  rdfs:comment "Rhythm games challenge players to follow the beat or rhythm of music tracks." ;
  rdfs:seeAlso <http://dbpedia.org/resource/Rhythm_game> ;
  schema:url <https://store.steampowered.com/tags/en/Rhythm/> .

steam:Roguelike a owl:Class, steam:Genre ;
  rdfs:label "Roguelike" ;
  rdfs:comment "Roguelike games feature procedurally generated levels and permadeath, often with RPG elements." ;
  rdfs:seeAlso <http://dbpedia.org/resource/Roguelike> ;
  schema:url <https://store.steampowered.com/tags/en/Roguelike/> .

steam:RTS a owl:Class, steam:Genre ;
  rdfs:label "RTS" ;
  rdfs:comment "Real-Time Strategy (RTS) games require strategic decision making in real time, often involving resource management and direct control over units." ;
  rdfs:subClassOf steam:Strategy ;
  rdfs:seeAlso <http://dbpedia.org/resource/Real-time_strategy> ;
  schema:url <https://store.steampowered.com/tags/en/RTS/> .

steam:Sandbox a owl:Class, steam:Genre ;
  rdfs:label "Sandbox" ;
  rdfs:comment "Sandbox games allow players to explore, create, and manipulate their environment with few imposed goals or restrictions." ;
  rdfs:seeAlso <http://dbpedia.org/resource/Sandbox_game> ;
  schema:url <https://store.steampowered.com/tags/en/Sandbox/> .

steam:Shooter a owl:Class, steam:Genre ;
  rdfs:label "Shooter" ;
  rdfs:comment "Shooter games focus on combat involving projectile weapons, such as guns and missiles." ;
  rdfs:subClassOf steam:Action ;
  rdfs:seeAlso <http://dbpedia.org/resource/Shooter_game> ;
  schema:url <https://store.steampowered.com/tags/en/Shooter/> .

steam:Skateboarding a owl:Class, steam:Genre ;
  rdfs:label "Skateboarding" ;
  rdfs:comment "Skateboarding games simulate skateboarding activities, often with a focus on performing tricks and stunts." ;
  rdfs:subClassOf steam:Skating ;
  rdfs:seeAlso <http://dbpedia.org/resource/Skateboarding> ;
  schema:url <https://store.steampowered.com/tags/en/Skateboarding/> .

steam:Skating a owl:Class, steam:Genre ;
  rdfs:label "Skating" ;
  rdfs:comment "Skating games simulate skating activities, often with a focus on performing tricks and stunts." ;
  rdfs:subClassOf steam:Sports ;
  rdfs:seeAlso <http://dbpedia.org/resource/Skating> ;
  schema:url <https://store.steampowered.com/tags/en/Skating/> .

steam:Skiing a owl:Class, steam:Genre ;
  rdfs:label "Skiing" ;
  rdfs:comment "Skiing games simulate skiing activities, often with a focus on racing or performing tricks." ;
  rdfs:subClassOf steam:Sports ;
  rdfs:seeAlso <http://dbpedia.org/resource/Skiing> ;
  schema:url <https://store.steampowered.com/tags/en/Skiing/> .

steam:Snowboarding a owl:Class, steam:Genre ;
  rdfs:label "Snowboarding" ;
  rdfs:comment "Snowboarding games simulate snowboarding activities, often with a focus on racing or performing tricks." ;
  rdfs:subClassOf steam:Sports ;
  rdfs:seeAlso <http://dbpedia.org/resource/Snowboarding> ;
  schema:url <https://store.steampowered.com/tags/en/Snowboarding/> .

steam:Soccer a owl:Class, steam:Genre ;
  rdfs:label "Soccer" ;
  rdfs:comment "Soccer games simulate the sport of soccer, often with a focus on controlling a team and competing in matches." ;
  rdfs:subClassOf steam:Sports ;
  rdfs:seeAlso <http://dbpedia.org/resource/Association_football> ;
  schema:url <https://store.steampowered.com/tags/en/Soccer/> .

steam:SpaceSim a owl:Class, steam:Genre ;
  rdfs:label "Space Sim" ;
  rdfs:comment "Space Sim games simulate space exploration or combat in a space setting." ;
  rdfs:subClassOf steam:Simulation ;
  rdfs:seeAlso <http://dbpedia.org/resource/Space_flight_simulation_game> ;
  schema:url <https://store.steampowered.com/tags/en/Space%20Sim/> .

steam:Stealth a owl:Class, steam:Genre ;
  rdfs:label "Stealth" ;
  rdfs:comment "Stealth games challenge players to avoid detection, often by sneaking past enemies or obstacles." ;
  rdfs:seeAlso <http://dbpedia.org/resource/Stealth_game> ;
  schema:url <https://store.steampowered.com/tags/en/Stealth/> .

steam:StrategyRPG a owl:Class, steam:Genre ;
  rdfs:label "Strategy RPG" ;
  rdfs:comment "Strategy RPGs combine strategic gameplay with role-playing elements, often involving character development and tactical combat." ;
  rdfs:subClassOf steam:RPG, steam:Strategy ;
  rdfs:seeAlso <http://dbpedia.org/resource/Tactical_role-playing_game> ;
  schema:url <https://store.steampowered.com/tags/en/Strategy%20RPG/> .

steam:Survival a owl:Class, steam:Genre ;
  rdfs:label "Survival" ;
  rdfs:comment "Survival games challenge players to survive in a hostile environment, often by gathering resources, crafting tools, and building shelters." ;
  rdfs:seeAlso <http://dbpedia.org/resource/Survival_game> ;
  schema:url <https://store.steampowered.com/tags/en/Survival/> .

steam:Tennis a owl:Class, steam:Genre ;
  rdfs:label "Tennis" ;
  rdfs:comment "Tennis games simulate the sport of tennis, often with a focus on controlling a player and competing in matches." ;
  rdfs:subClassOf steam:Sports ;
  rdfs:seeAlso <http://dbpedia.org/resource/Tennis> ;
  schema:url <https://store.steampowered.com/tags/en/Tennis/> .

steam:TowerDefense a owl:Class, steam:Genre ;
  rdfs:label "Tower Defense" ;
  rdfs:comment "Tower Defense games challenge players to defend a location by placing defensive structures along the path of incoming enemies." ;
  rdfs:subClassOf steam:Strategy ;
  rdfs:seeAlso <http://dbpedia.org/resource/Tower_defense> ;
  schema:url <https://store.steampowered.com/tags/en/Tower%20Defense/> .

steam:Trivia a owl:Class, steam:Genre ;
  rdfs:label "Trivia" ;
  rdfs:comment "Trivia games test players' knowledge of various topics, often in a quiz format." ;
  rdfs:subClassOf steam:Casual ;
  rdfs:seeAlso <http://dbpedia.org/resource/Trivia> ;
  schema:url <https://store.steampowered.com/tags/en/Trivia/> .

steam:TurnBasedStrategy a owl:Class, steam:Genre ;
  rdfs:label "Turn-Based Strategy" ;
  rdfs:comment "Turn-Based Strategy games involve strategic gameplay where players take turns when playing." ;
  rdfs:subClassOf steam:Strategy ;
  rdfs:seeAlso <http://dbpedia.org/resource/Turn-based_strategy> ;
  schema:url <https://store.steampowered.com/tags/en/Turn-Based%20Strategy/> .

steam:VisualNovel a owl:Class, steam:Genre ;
  rdfs:label "Visual Novel" ;
  rdfs:comment "Visual Novels are a narrative genre of game, featuring mostly static graphics, most often using anime-style art or occasionally live-action stills." ;
  rdfs:seeAlso <http://dbpedia.org/resource/Visual_novel> ;
  schema:url <https://store.steampowered.com/tags/en/Visual%20Novel/> .

steam:WalkingSimulator a owl:Class, steam:Genre ;
  rdfs:label "Walking Simulator" ;
  rdfs:comment "Walking Simulator games focus on exploration and narrative over gameplay, often involving walking through an environment to uncover the story." ;
  rdfs:subClassOf steam:Adventure ;
  schema:url <https://store.steampowered.com/tags/en/Walking%20Simulator/> .

steam:WordGame a owl:Class, steam:Genre ;
  rdfs:label "Word Game" ;
  rdfs:comment "Word games involve the creation or solving of words, often in a puzzle format." ;
  rdfs:subClassOf steam:Puzzle, steam:Casual ;
  rdfs:seeAlso <http://dbpedia.org/resource/Word_game> ;
  schema:url <https://store.steampowered.com/tags/en/Word%20Game/> .

steam:Wrestling a owl:Class, steam:Genre ;
  rdfs:label "Wrestling" ;
  rdfs:comment "Wrestling games simulate the sport of wrestling, often with a focus on controlling a wrestler and competing in matches." ;
  rdfs:subClassOf steam:Sports ;
  rdfs:seeAlso <http://dbpedia.org/resource/Professional_wrestling> ;
  schema:url <https://store.steampowered.com/tags/en/Wrestling/> .

# Sub-Genre tags

steam:2DFighter a owl:Class, steam:SubGenre ;
  rdfs:label "2D Fighter" ;
  rdfs:comment "2D Fighter games are fighting games with a gameplay in a two-dimensional environment." ;
  rdfs:subClassOf steam:Fighting ;
  schema:url <https://store.steampowered.com/tags/en/2D%20Fighter/> .

steam:2DPlatformer a owl:Class, steam:SubGenre ;
  rdfs:label "2D Platformer" ;
  rdfs:comment "2D Platformer games are platform games with a gameplay in a two-dimensional environment." ;
  rdfs:subClassOf steam:Platformer ;
  schema:url <https://store.steampowered.com/tags/en/2D%20Platformer/> .

steam:3DFighter a owl:Class, steam:SubGenre ;
  rdfs:label "3D Fighter" ;
  rdfs:comment "3D Fighter games are fighting games with a gameplay in a three-dimensional environment." ;
  rdfs:subClassOf steam:Fighting ;
  schema:url <https://store.steampowered.com/tags/en/3D%20Fighter/> .

steam:3DPlatformer a owl:Class, steam:SubGenre ;
  rdfs:label "3D Platformer" ;
  rdfs:comment "3D Platformer games are platform games with a gameplay in a three-dimensional environment." ;
  rdfs:subClassOf steam:Platformer ;
  schema:url <https://store.steampowered.com/tags/en/3D%20Platformer/> .

steam:4X a owl:Class, steam:SubGenre ;
  rdfs:label "4X" ;
  rdfs:comment "4X games are a genre of strategy video game in which players control an empire and 'eXplore, eXpand, eXploit, and eXterminate'." ;
  rdfs:subClassOf steam:Strategy ;
  rdfs:seeAlso <http://dbpedia.org/resource/4X> ;
  schema:url <https://store.steampowered.com/tags/en/4X/> .

steam:ActionRoguelike a owl:Class, steam:SubGenre ;
  rdfs:label "Action Roguelike" ;
  rdfs:comment "Action Roguelike games combine the action genre with roguelike elements, including procedural generation and permadeath." ;
  rdfs:subClassOf steam:Roguelike ;
  schema:url <https://store.steampowered.com/tags/en/Action%20Roguelike/> .

steam:ArenaShooter a owl:Class, steam:SubGenre ;
  rdfs:label "Arena Shooter" ;
  rdfs:comment "Arena Shooter games are shooter games that take place in contained arena environments, often with a focus on multiplayer combat." ;
  rdfs:subClassOf steam:Shooter ;
  rdfs:seeAlso <http://dbpedia.org/resource/Shooter_game> ;
  schema:url <https://store.steampowered.com/tags/en/Arena%20Shooter/> .

steam:BeatEmUp a owl:Class, steam:SubGenre ;
  rdfs:label "Beat 'em up" ;
  rdfs:comment "Beat 'em up games are action games that feature hand-to-hand combat between the protagonist and an improbably large number of opponents." ;
  rdfs:subClassOf steam:Action ;
  schema:url <https://store.steampowered.com/tags/en/Beat%20'Em%20Up/> .

steam:BulletHell a owl:Class, steam:SubGenre ;
  rdfs:label "Bullet Hell" ;
  rdfs:comment "Bullet Hell games are shooting games that feature overwhelming numbers of enemy projectiles, often in visually impressive patterns." ;
  rdfs:subClassOf steam:ShootEmUp ;
  schema:url <https://store.steampowered.com/tags/en/Bullet%20Hell/> .

steam:CardBattler a owl:Class, steam:SubGenre ;
  rdfs:label "Card Battler" ;
  rdfs:comment "Card Battler games are games that use cards as a primary element to let players strategize and compete against each other." ;
  rdfs:subClassOf steam:CardGame ;
  schema:url <https://store.steampowered.com/tags/en/Card%20Battler/> .

steam:ChooseYourOwnAdventure a owl:Class, steam:SubGenre ;
  rdfs:label "Choose Your Own Adventure" ;
  rdfs:comment "Choose Your Own Adventure games are games that feature interactive stories where the player can make choices that affect the outcome." ;
  rdfs:subClassOf steam:Adventure ;
  rdfs:seeAlso <http://dbpedia.org/resource/Gamebook> ;
  schema:url <https://store.steampowered.com/tags/en/Choose%20Your%20Own%20Adventure/> .

steam:CityBuilder a owl:Class, steam:SubGenre ;
  rdfs:label "City Builder" ;
  rdfs:comment "City Builder games are a type of simulation game where players build, expand and manage fictional communities or projects with limited resources." ;
  rdfs:subClassOf steam:Simulation ;
  rdfs:seeAlso <http://dbpedia.org/resource/City-building_game> ;
  schema:url <https://store.steampowered.com/tags/en/City%20Builder/> .

steam:Collectathon a owl:Class, steam:SubGenre ;
  rdfs:label "Collectathon" ;
  rdfs:comment "Collectathon games are games that feature collecting a large number of items as a core mechanic." ;
  schema:url <https://store.steampowered.com/tags/en/Collectathon/> .

steam:ColonySim a owl:Class, steam:SubGenre ;
  rdfs:label "Colony Sim" ;
  rdfs:comment "Colony Sim games are a type of simulation game where players build, expand and manage a colony or project with limited resources." ;
  rdfs:subClassOf steam:Simulation ;
  schema:url <https://store.steampowered.com/tags/en/Colony%20Sim/> .

steam:CombatRacing a owl:Class, steam:SubGenre ;
  rdfs:label "Combat Racing" ;
  rdfs:comment "Combat Racing games are racing games that feature combat elements, such as weapons or aggressive driving maneuvers." ;
  rdfs:subClassOf steam:Racing, steam:Action ;
  rdfs:seeAlso <http://dbpedia.org/resource/List_of_vehicular_combat_games> ;
  schema:url <https://store.steampowered.com/tags/en/Combat%20Racing/> .

steam:CRPG a owl:Class, steam:SubGenre ;
  rdfs:label "CRPG" ;
  rdfs:comment "CRPG (Computer Role-Playing Games) are a type of role-playing video game which are played on a computer and use similar mechanics to traditional tabletop RPGs." ;
  rdfs:subClassOf steam:RPG ;
  schema:url <https://store.steampowered.com/tags/en/CRPG/> .

steam:DatingSim a owl:Class, steam:SubGenre ;
  rdfs:label "Dating Sim" ;
  rdfs:comment "Dating Sim games are a type of simulation game where players simulate romantic or sexual relationships. They often involve dialogues and character development." ;
  rdfs:subClassOf steam:Simulation ;
  rdfs:seeAlso <http://dbpedia.org/resource/Dating_sim> ;
  schema:url <https://store.steampowered.com/tags/en/Dating%20Sim/> .

steam:DungeonCrawler a owl:Class, steam:SubGenre ;
  rdfs:label "Dungeon Crawler" ;
  rdfs:comment "Dungeon Crawler games are a type of adventure games where players navigate a labyrinth environment, battling various monsters, and looting any treasure they may find." ;
  rdfs:subClassOf steam:Adventure ;
  rdfs:seeAlso <http://dbpedia.org/resource/Dungeon_crawl> ;
  schema:url <https://store.steampowered.com/tags/en/Dungeon%20Crawler/> .

steam:Education a owl:Class, steam:SubGenre ;
  rdfs:label "Education" ;
  rdfs:comment "Education games are designed to teach people about certain subjects, expand concepts, reinforce development, or assist them in learning a skill as they play." ;
  rdfs:seeAlso <http://dbpedia.org/resource/Educational_game> ;
  schema:url <https://store.steampowered.com/tags/en/Education/> .

steam:Flight a owl:Class, steam:SubGenre ;
  rdfs:label "Flight" ;
  rdfs:comment "Flight games are games that involve piloting a vehicle, often an aircraft, through the sky." ;
  rdfs:subClassOf steam:Simulation ;
  rdfs:seeAlso <http://dbpedia.org/resource/Flight_simulator> ;
  schema:url <https://store.steampowered.com/tags/en/Flight/> .

steam:FPS a owl:Class, steam:SubGenre ;
  rdfs:label "FPS" ;
  rdfs:comment "FPS (First-Person Shooter) games are a type of 3D shooter games played from a first-person perspective, where the player experiences the action through the eyes of the protagonist." ;
  rdfs:subClassOf steam:Shooter ;
  rdfs:seeAlso <http://dbpedia.org/resource/First-person_shooter> ;
  schema:url <https://store.steampowered.com/tags/en/FPS/> .

steam:GrandStrategy a owl:Class, steam:SubGenre ;
  rdfs:label "Grand Strategy" ;
  rdfs:comment "Grand Strategy games are a type of strategy game that includes aspects of military, economic, and political development. Players control a nation or faction and make long-term strategic decisions." ;
  rdfs:subClassOf steam:Strategy ;
  rdfs:seeAlso <http://dbpedia.org/resource/Grand_strategy_wargame> ;
  schema:url <https://store.steampowered.com/tags/en/Grand%20Strategy/> .

steam:HackAndSlash a owl:Class, steam:SubGenre ;
  rdfs:label "Hack and Slash" ;
  rdfs:comment "Hack and Slash games are a type of action game that emphasizes combat with melee-based weapons." ;
  rdfs:subClassOf steam:Action ;
  rdfs:seeAlso <http://dbpedia.org/resource/Hack_and_slash> ;
  schema:url <https://store.steampowered.com/tags/en/Hack%20and%20Slash/> .

steam:Heist a owl:Class, steam:SubGenre ;
  rdfs:label "Heist" ;
  rdfs:comment "Heist games are games that involve a plot to commit a burglary or theft of some kind." ;
  rdfs:subClassOf steam:Action ;
  rdfs:seeAlso <http://dbpedia.org/resource/Heist_film> ;
  schema:url <https://store.steampowered.com/tags/en/Heist/> .

steam:HeroShooter a owl:Class, steam:SubGenre ;
  rdfs:label "Hero Shooter" ;
  rdfs:comment "Hero Shooter games are a sub-genre of shooter games that assign players into two or more teams, with each player selecting their own unique 'hero' character, each with their own unique abilities or skills." ;
  rdfs:subClassOf steam:Shooter ;
  rdfs:seeAlso <http://dbpedia.org/resource/Hero_shooter> ;
  schema:url <https://store.steampowered.com/tags/en/Hero%20Shooter/> .

steam:Horror a owl:Class, steam:SubGenre ;
  rdfs:label "Horror" ;
  rdfs:comment "Horror games are games that aim to elicit fear and horror from the player. They often feature dark atmospheres, scary graphics, and chilling audio." ;
  rdfs:seeAlso <http://dbpedia.org/resource/Category:Horror_video_games> ;
  schema:url <https://store.steampowered.com/tags/en/Horror/> .

steam:ImmersiveSim a owl:Class, steam:SubGenre ;
  rdfs:label "Immersive Sim" ;
  rdfs:comment "Immersive Sim games are a type of video game that emphasizes player choice. Their key defining features are a blend of multiple gameplay genres, and a highly interactive world." ;
  rdfs:subClassOf steam:Simulation ;
  rdfs:seeAlso <http://dbpedia.org/resource/Immersive_sim> ;
  schema:url <https://store.steampowered.com/tags/en/Immersive%20Sim/> .

steam:Investigation a owl:Class, steam:SubGenre ;
  rdfs:label "Investigation" ;
  rdfs:comment "The Investigation tag is used for games that might involve solving mysteries, uncovering clues, or playing as a detective or investigator." ;
  rdfs:seeAlso <http://dbpedia.org/resource/Detective_fiction> ;
  schema:url <https://store.steampowered.com/tags/en/Investigation/> .

steam:JRPG a owl:Class, steam:SubGenre ;
  rdfs:label "JRPG" ;
  rdfs:comment "JRPG (Japanese Role-Playing Games) are a type of role-playing video game that originated in Japan and have a distinct art style and narrative structure." ;
  rdfs:subClassOf steam:RPG ;
  rdfs:seeAlso <http://dbpedia.org/resource/History_of_Eastern_role-playing_video_games> ;
  schema:url <https://store.steampowered.com/tags/en/JRPG/> .

steam:LifeSim a owl:Class, steam:SubGenre ;
  rdfs:label "Life Sim" ;
  rdfs:comment "Life Sim games are a type of simulation game where players simulate living or controlling one or more artificial lives." ;
  rdfs:subClassOf steam:Simulation ;
  rdfs:seeAlso <http://dbpedia.org/resource/Life_simulation_game> ;
  schema:url <https://store.steampowered.com/tags/en/Life%20Sim/> .

steam:LooterShooter a owl:Class, steam:SubGenre ;
  rdfs:label "Looter Shooter" ;
  rdfs:comment "Looter Shooter games are a sub-genre of shooter games that include elements of looting, shooting, and often role-playing." ;
  rdfs:subClassOf steam:Shooter ;
  schema:url <https://store.steampowered.com/tags/en/Looter%20Shooter/> .

steam:Metroidvania a owl:Class, steam:SubGenre ;
  rdfs:label "Metroidvania" ;
  rdfs:comment "Metroidvania games are a sub-genre of action-adventure games that includes elements of exploration, backtracking, and item gathering." ;
  rdfs:subClassOf steam:Action, steam:Platformer ;
  rdfs:seeAlso <http://dbpedia.org/resource/Metroidvania> ;
  schema:url <https://store.steampowered.com/tags/en/Metroidvania/> .

steam:MysteryDungeon a owl:Class, steam:SubGenre ;
  rdfs:label "Mystery Dungeon" ;
  rdfs:comment "Mystery Dungeon games are a sub-genre of role-playing games that feature randomly generated dungeons and turn-based combat." ;
  rdfs:subClassOf [ a owl:Class ; owl:intersectionOf ( steam:RPG steam:Roguelike ) ] ;
  rdfs:seeAlso <http://dbpedia.org/resource/Mystery_Dungeon> ;
  schema:url <https://store.steampowered.com/tags/en/Mystery%20Dungeon/> .

steam:OnRailsShooter a owl:Class, steam:SubGenre ;
  rdfs:label "On-Rails Shooter" ;
  rdfs:comment "On-Rails Shooter games are a type of shooter game where the player's movement is automatically guided along a fixed path, or 'on rails'." ;
  rdfs:subClassOf steam:Shooter ;
  schema:url <https://store.steampowered.com/tags/en/On-Rails%20Shooter/> .

steam:OpenWorldSurvivalCraft a owl:Class, steam:SubGenre ;
  rdfs:label "Open World Survival Craft" ;
  rdfs:comment "Open World Survival Craft games are a type of survival game where players must gather resources, build their own items, and manage their needs, all while exploring an open world." ;
  rdfs:subClassOf steam:Survival, steam:OpenWorld ;
  schema:url <https://store.steampowered.com/tags/en/Open%20World%20Survival%20Craft/> .

steam:PoliticalSim a owl:Class, steam:SubGenre ;
  rdfs:label "Political Sim" ;
  rdfs:comment "Political Sim games are a type of simulation game where players simulate the politics and government of a nation or civilization." ;
  rdfs:subClassOf steam:Simulation ;
  rdfs:seeAlso <http://dbpedia.org/resource/Government_simulation_game> ;
  schema:url <https://store.steampowered.com/tags/en/Political%20Sim/> .

steam:PrecisionPlatformer a owl:Class, steam:SubGenre ;
  rdfs:label "Precision Platformer" ;
  rdfs:comment "Precision Platformer games are a sub-genre of platformer games that require precise control and timing." ;
  rdfs:subClassOf steam:Platformer ;
  schema:url <https://store.steampowered.com/tags/en/Precision%20Platformer/> .

steam:Programming a owl:Class, steam:SubGenre ;
  rdfs:label "Programming" ;
  rdfs:comment "Programming games are games where the player has limited direct control over the game characters, and completes levels or achieves goals by programming game elements." ;
  rdfs:subClassOf steam:Simulation ;
  rdfs:seeAlso <http://dbpedia.org/resource/Programming_game> ;
  schema:url <https://store.steampowered.com/tags/en/Programming/> .

steam:RealTimeTactics a owl:Class, steam:SubGenre ;
  rdfs:label "Real Time Tactics" ;
  rdfs:comment "Real Time Tactics games are a type of strategy game that focuses on tactical and operational aspects of warfare, as opposed to strategic or grand strategy." ;
  rdfs:subClassOf steam:Strategy ;
  rdfs:seeAlso <http://dbpedia.org/resource/Real-time_tactics> ;
  schema:url <https://store.steampowered.com/tags/en/Real%20Time%20Tactics/> .

steam:Roguelite a owl:Class, steam:SubGenre ;
  rdfs:label "Roguelite" ;
  rdfs:comment "Roguelite games feature procedurally generated levels, permadeath, and other elements of roguelikes. They are characterized by their difficulty and replayability." ;
  rdfs:subClassOf steam:Roguelike ;
  schema:url <https://store.steampowered.com/tags/en/Roguelite/> .

steam:Roguevania a owl:Class, steam:SubGenre ;
  rdfs:label "Roguevania" ;
  rdfs:comment "Roguevania games are a sub-genre of action-adventure games that combine elements of roguelike and metroidvania games." ;
  rdfs:subClassOf [ a owl:Class ; owl:intersectionOf ( steam:Roguelike steam:Metroidvania ) ] ;
  schema:url <https://store.steampowered.com/tags/en/Roguevania/> .

steam:Runner a owl:Class, steam:SubGenre ;
  rdfs:label "Runner" ;
  rdfs:comment "Runner games are a type of action game where the player character is continuously moving forward and the player must control their actions to avoid obstacles and collect items." ;
  rdfs:subClassOf steam:Action ;
  schema:url <https://store.steampowered.com/tags/en/Runner/> .

steam:ShootEmUp a owl:Class, steam:SubGenre ;
  rdfs:label "Shoot 'Em Up" ;
  rdfs:comment "Shoot 'Em Up games are a sub-genre of shooter games where the player controls a character or vehicle and fights large numbers of enemies using shooting." ;
  rdfs:subClassOf steam:Shooter ;
  rdfs:seeAlso <http://dbpedia.org/resource/Shoot_'em_up> ;
  schema:url <https://store.steampowered.com/tags/en/Shoot%20'Em%20Up/> .

steam:SideScroller a owl:Class, steam:SubGenre ;
  rdfs:label "Side Scroller" ;
  rdfs:comment "Side Scroller games are a type of game in which gameplay is viewed from a side-view camera angle, and the characters move from the left side of the screen to the right (or vice versa)." ;
  rdfs:seeAlso <http://dbpedia.org/resource/Side-scrolling_video_game> ;
  schema:url <https://store.steampowered.com/tags/en/Side%20Scroller/> .

steam:Sokoban a owl:Class, steam:SubGenre ;
  rdfs:label "Sokoban" ;
  rdfs:comment "Sokoban games are a type of puzzle game where the player pushes boxes or crates around in a warehouse, trying to get them to storage locations." ;
  rdfs:subClassOf steam:Puzzle ;
  rdfs:seeAlso <http://dbpedia.org/resource/Sokoban> ;
  schema:url <https://store.steampowered.com/tags/en/Sokoban/> .

steam:Solitaire a owl:Class, steam:SubGenre ;
  rdfs:label "Solitaire" ;
  rdfs:comment "Solitaire games are a type of card game that can be played by a single player." ;
  rdfs:subClassOf steam:CardGame ;
  rdfs:subClassOf [
    a owl:Restriction ;
    owl:onProperty schema:playMode ;
    owl:hasValue schema:SinglePlayer
    ] ;
  rdfs:seeAlso <http://dbpedia.org/resource/Solitaire> ;
  schema:url <https://store.steampowered.com/tags/en/Solitaire/> .

steam:SoulsLike a owl:Class, steam:SubGenre ;
  rdfs:label "Souls-like" ;
  rdfs:comment "Souls-like games are a sub-genre of action RPGs that include elements of challenging combat, exploration, and character development, inspired by the Dark Souls series." ;
  rdfs:subClassOf steam:ActionRPG ;
  rdfs:seeAlso <http://dbpedia.org/resource/Souls_(series)> ;
  schema:url <https://store.steampowered.com/tags/en/Souls-like/> .

steam:SpectacleFighter a owl:Class, steam:SubGenre ;
  rdfs:label "Spectacle Fighter" ;
  rdfs:comment "Spectacle Fighter games are a sub-genre of action games that feature fast-paced combat with flashy, over-the-top attacks and combos." ;
  rdfs:subClassOf steam:Fighting ;
  schema:url <https://store.steampowered.com/tags/en/Spectacle%20Fighter/> .

steam:Spelling a owl:Class, steam:SubGenre ;
  rdfs:label "Spelling" ;
  rdfs:comment "Spelling games are a type of educational game that focuses on the correct spelling of words." ;
  rdfs:subClassOf steam:Education ;
  schema:url <https://store.steampowered.com/tags/en/Spelling/> .

steam:SurvivalHorror a owl:Class, steam:SubGenre ;
  rdfs:label "Survival Horror" ;
  rdfs:comment "Survival Horror games are a sub-genre of horror games that focus on survival of the character and the fear of the unknown." ;
  rdfs:subClassOf [ a owl:Class ; owl:intersectionOf ( steam:Horror steam:Survival ) ] ;
  rdfs:seeAlso <http://dbpedia.org/resource/Survival_horror> ;
  schema:url <https://store.steampowered.com/tags/en/Survival%20Horror/> .

steam:TacticalRPG a owl:Class, steam:SubGenre ;
  rdfs:label "Tactical RPG" ;
  rdfs:comment "Tactical RPG games are a sub-genre of role-playing games that focus on tactical and strategic battles, often using turn-based combat." ;
  rdfs:subClassOf [ a owl:Class ; owl:intersectionOf ( steam:RPG steam:Strategy ) ] ;
  rdfs:seeAlso <http://dbpedia.org/resource/Tactical_role-playing_game> ;
  schema:url <https://store.steampowered.com/tags/en/Tactical%20RPG/> .

steam:ThirdPersonShooter a owl:Class, steam:SubGenre ;
  rdfs:label "Third-Person Shooter" ;
  rdfs:comment "Third-Person Shooter games are a sub-genre of shooter games where the player views the game from a third-person perspective, usually behind the character they are controlling." ;
  rdfs:subClassOf steam:Shooter ;
  rdfs:seeAlso <http://dbpedia.org/resource/Third-person_shooter> ;
  schema:url <https://store.steampowered.com/tags/en/Third-Person%20Shooter/> .

steam:TimeManagement a owl:Class, steam:SubGenre ;
  rdfs:label "Time Management" ;
  rdfs:comment "Time Management games are a sub-genre of strategy games that require the player to complete specific tasks within a certain timeframe to succeed." ;
  rdfs:subClassOf steam:Strategy ;
  schema:url <https://store.steampowered.com/tags/en/Time%20Management/> .

steam:TopDownShooter a owl:Class, steam:SubGenre ;
  rdfs:label "Top-Down Shooter" ;
  rdfs:comment "Top-Down Shooter games are a sub-genre of shooter games where the player views the game from a top-down perspective, shooting enemies and avoiding obstacles from this viewpoint." ;
  rdfs:subClassOf steam:Shooter ;
  schema:url <https://store.steampowered.com/tags/en/Top-Down%20Shooter/> .

steam:Trading a owl:Class, steam:SubGenre ;
  rdfs:label "Trading" ;
  rdfs:comment "Trading games are a type of game that focuses on trading goods and services, often in an economic simulation context." ;
  schema:url <https://store.steampowered.com/tags/en/Trading/> .

steam:TradingCardGame a owl:Class, steam:SubGenre ;
  rdfs:label "Trading Card Game" ;
  rdfs:comment "Trading Card Game games are a type of card game where players use collectible cards to strategize and defeat their opponents." ;
  rdfs:subClassOf steam:CardGame ;
  rdfs:seeAlso <http://dbpedia.org/resource/Collectible_card_game> ;
  schema:url <https://store.steampowered.com/tags/en/Trading%20Card%20Game/> .

steam:TraditionalRoguelike a owl:Class, steam:SubGenre ;
  rdfs:label "Traditional Roguelike" ;
  rdfs:comment "Traditional Roguelike games are a sub-genre of roguelike games that adhere closely to the original roguelike design, featuring turn-based combat, grid-based movement, and permadeath." ;
  rdfs:subClassOf steam:Roguelike ;
  schema:url <https://store.steampowered.com/tags/en/Traditional%20Roguelike/> .

steam:TurnBasedTactics a owl:Class, steam:SubGenre ;
  rdfs:label "Turn-Based Tactics" ;
  rdfs:comment "Turn-Based Tactics games are a type of strategy game that features tactical combat in which players take turns to command their units." ;
  rdfs:subClassOf steam:TurnBasedStrategy ;
  rdfs:seeAlso <http://dbpedia.org/resource/Turn-based_tactics> ;
  schema:url <https://store.steampowered.com/tags/en/Turn-Based%20Tactics/> .

steam:TwinStickShooter a owl:Class, steam:SubGenre ;
  rdfs:label "Twin Stick Shooter" ;
  rdfs:comment "Twin Stick Shooter games are a sub-genre of shooter games that use a dual-stick control scheme, where one stick controls movement and the other controls the direction of shooting." ;
  rdfs:subClassOf steam:Shooter ;
  schema:url <https://store.steampowered.com/tags/en/Twin%20Stick%20Shooter/> .

steam:Typing a owl:Class, steam:SubGenre ;
  rdfs:label "Typing" ;
  rdfs:comment "Typing games are a type of educational game that focuses on typing skills. Players are often tasked with typing words or phrases correctly and quickly to achieve goals in the game." ;
  rdfs:subClassOf steam:Education ;
  schema:url <https://store.steampowered.com/tags/en/Typing/> .

steam:Wargame a owl:Class, steam:SubGenre ;
  rdfs:label "Wargame" ;
  rdfs:comment "Wargame games are a type of strategy game that simulates warfare. They often focus on realistic tactical and strategic battles, and can cover various periods of history." ;
  rdfs:subClassOf steam:Strategy ;
  rdfs:seeAlso <http://dbpedia.org/resource/Computer_wargame> ;
  schema:url <https://store.steampowered.com/tags/en/Wargame/> .

# Visuals and Viewpoint tag classes

steam:2.5D a owl:Class, steam:VisualsAndViewpoint ;
  rdfs:label "2.5D" ;
  rdfs:comment "2.5D is a visual style that combines 2D graphics with a 3D perspective. This is often done to create depth or to achieve certain visual effects." ;
  rdfs:seeAlso <http://dbpedia.org/resource/2.5D> ;
  schema:url <https://store.steampowered.com/tags/en/2.5D/> .

steam:2D a owl:Class, steam:VisualsAndViewpoint ;
  rdfs:label "2D" ;
  rdfs:comment "2D is a visual style that uses two-dimensional graphics. This often includes side-scrolling elements, platformers, and top-down perspectives." ;
  rdfs:seeAlso <http://dbpedia.org/resource/2D_computer_graphics> ;
  schema:url <https://store.steampowered.com/tags/en/2D/> .

steam:360Video a owl:Class, steam:VisualsAndViewpoint ;
  rdfs:label "360 Video" ;
  rdfs:comment "360 Video is a type of media that features 360-degree videos, allowing the viewer to look in any direction. This is often used in virtual reality experiences." ;
  rdfs:seeAlso <http://dbpedia.org/resource/360-degree_video> ;
  schema:url <https://store.steampowered.com/tags/en/360%20Video/> .

steam:3D a owl:Class, steam:VisualsAndViewpoint ;
  rdfs:label "3D" ;
  rdfs:comment "3D is a visual style that uses three-dimensional graphics. This can include a wide variety of media, from games to movies, and is used to create a sense of depth and realism." ;
  rdfs:seeAlso <http://dbpedia.org/resource/3D_computer_graphics> ;
  schema:url <https://store.steampowered.com/tags/en/3D/> .

steam:3DVision a owl:Class, steam:VisualsAndViewpoint ;
  rdfs:label "3D Vision" ;
  rdfs:comment "3D Vision is a technology that supports Nvidia's 3D Vision technology, which allows for stereoscopic viewing on 3D monitors and TVs." ;
  rdfs:seeAlso <http://dbpedia.org/resource/Nvidia_3D_Vision> ;
  schema:url <https://store.steampowered.com/tags/en/3D%20Vision/> .

steam:Abstract a owl:Class, steam:VisualsAndViewpoint ;
  rdfs:label "Abstract" ;
  rdfs:comment "Abstract refers to a visual style that does not attempt to represent an accurate depiction of visual reality. It uses shapes, colors, forms and gestural marks to achieve its effect." ;
  rdfs:seeAlso <http://dbpedia.org/resource/Abstract_art> ;
  schema:url <https://store.steampowered.com/tags/en/Abstract/> .

steam:Anime a owl:Class, steam:VisualsAndViewpoint ;
  rdfs:label "Anime" ;
  rdfs:comment "Anime is a style of animation originating from Japan, characterized by colorful artwork, fantastical themes, and vibrant characters." ;
  rdfs:seeAlso <http://dbpedia.org/resource/Anime> ;
  schema:url <https://store.steampowered.com/tags/en/Anime/> .

steam:Cartoon a owl:Class, steam:VisualsAndViewpoint ;
  rdfs:label "Cartoon" ;
  rdfs:comment "Cartoon is a style of drawing that is typically non-realistic or semi-realistic artistic style, often used in animations and graphic novels." ;
  rdfs:seeAlso <http://dbpedia.org/resource/Cartoon> ;
  schema:url <https://store.steampowered.com/tags/en/Cartoon/> .

steam:Cartoony a owl:Class, steam:VisualsAndViewpoint ;
  rdfs:label "Cartoony" ;
  rdfs:comment "Cartoony is a visual style that resembles traditional cartoon aesthetics, often characterized by exaggerated features, bright colors, and a lack of realistic details." ;
  schema:url <https://store.steampowered.com/tags/en/Cartoony/> .

steam:Cinematic a owl:Class, steam:VisualsAndViewpoint ;
  rdfs:label "Cinematic" ;
  rdfs:comment "Cinematic refers to a visual style that resembles the aesthetics of movies, often characterized by high-quality graphics, dramatic lighting, and camera angles." ;
  rdfs:seeAlso <http://dbpedia.org/resource/Cinematic_techniques> ;
  schema:url <https://store.steampowered.com/tags/en/Cinematic/> .

steam:Colorful a owl:Class, steam:VisualsAndViewpoint ;
  rdfs:label "Colorful" ;
  rdfs:comment "Colorful refers to a visual style that uses a wide range of colors, often in a vibrant and eye-catching manner." ;
  schema:url <https://store.steampowered.com/tags/en/Colorful/> .

steam:ComicBook a owl:Class, steam:VisualsAndViewpoint ;
  rdfs:label "Comic Book" ;
  rdfs:comment "The Comic Book tag is used for games that draw inspiration from the world of comic books. These games might feature bold, colorful art styles, larger-than-life characters, or narrative structures inspired by comic book storytelling." ;
  rdfs:seeAlso <http://dbpedia.org/resource/Comic_book> ;
  schema:url <https://store.steampowered.com/tags/en/Comic%20Book/> .

steam:Cute a owl:Class, steam:VisualsAndViewpoint ;
  rdfs:label "Cute" ;
  rdfs:comment "Cute is a visual style that is designed to be adorable and charming, often characterized by soft colors, round shapes, and endearing characters." ;
  schema:url <https://store.steampowered.com/tags/en/Cute/> .

steam:FirstPerson a owl:Class, steam:VisualsAndViewpoint ;
  rdfs:label "First-Person" ;
  rdfs:comment "First-Person refers to a perspective in which the audience experiences the world directly through the eyes of the character." ;
  rdfs:seeAlso <http://dbpedia.org/resource/First-person_(video_games)> ;
  schema:url <https://store.steampowered.com/tags/en/First-Person/> .

steam:FMV a owl:Class, steam:VisualsAndViewpoint ;
  rdfs:label "FMV" ;
  rdfs:comment "FMV, or Full Motion Video, refers to a technique used in video games that features pre-recorded video files (rather than sprites, vectors, or 3D models) to display action." ;
  rdfs:seeAlso <http://dbpedia.org/resource/Full_motion_video> ;
  schema:url <https://store.steampowered.com/tags/en/FMV/> .

steam:HandDrawn a owl:Class, steam:VisualsAndViewpoint ;
  rdfs:label "Hand-drawn" ;
  rdfs:comment "Hand-drawn refers to a visual style that appears to have been created by hand, often characterized by unique textures, lines, and colors that resemble traditional art mediums." ;
  schema:url <https://store.steampowered.com/tags/en/Hand-drawn/> .

steam:Isometric a owl:Class, steam:VisualsAndViewpoint ;
  rdfs:label "Isometric" ;
  rdfs:comment "Isometric refers to a method of drawing a three-dimensional object in two dimensions, where the three coordinate axes appear equally foreshortened." ;
  rdfs:seeAlso <http://dbpedia.org/resource/Isometric_video_game_graphics> ;
  schema:url <https://store.steampowered.com/tags/en/Isometric/> .

steam:Minimalist a owl:Class, steam:VisualsAndViewpoint ;
  rdfs:label "Minimalist" ;
  rdfs:comment "Minimalist refers to a visual style that is stripped down to its essential elements, often characterized by simplicity and the use of minimal colors, shapes, and textures." ;
  rdfs:seeAlso <http://dbpedia.org/resource/Minimalism> ;
  schema:url <https://store.steampowered.com/tags/en/Minimalist/> .

steam:Noir a owl:Class, steam:VisualsAndViewpoint ;
  rdfs:label "Noir" ;
  rdfs:comment "Noir is a visual style that is characterized by cynicism, fatalism, and moral ambiguity. It often uses a black-and-white aesthetic with high contrast and dramatic shadows." ;
  rdfs:seeAlso <http://dbpedia.org/resource/Film_noir> ;
  schema:url <https://store.steampowered.com/tags/en/Noir/> .

steam:PixelGraphics a owl:Class, steam:VisualsAndViewpoint ;
  rdfs:label "Pixel Graphics" ;
  rdfs:comment "Pixel Graphics refers to a visual style that uses pixel art, where images are created on the pixel level. This style is often associated with early video games." ;
  rdfs:seeAlso <http://dbpedia.org/resource/Pixel_art> ;
  schema:url <https://store.steampowered.com/tags/en/Pixel%20Graphics/> .

steam:Psychedelic a owl:Class, steam:VisualsAndViewpoint ;
  rdfs:label "Psychedelic" ;
  rdfs:comment "Psychedelic is a visual style that is characterized by the distortion of reality, vibrant colors, and complex, often surreal imagery." ;
  rdfs:seeAlso <http://dbpedia.org/resource/Psychedelia> ;
  schema:url <https://store.steampowered.com/tags/en/Psychedelic/> .

steam:Realistic a owl:Class, steam:VisualsAndViewpoint ;
  rdfs:label "Realistic" ;
  rdfs:comment "Realistic refers to a visual style that attempts to represent the physical world in a realistic manner. It often features detailed textures, accurate lighting, and complex models." ;
  schema:url <https://store.steampowered.com/tags/en/Realistic/> .

steam:SplitScreen a owl:Class, steam:VisualsAndViewpoint ;
  rdfs:label "Split Screen" ;
  rdfs:comment "Split Screen refers to a display technique that divides the screen into two or more parts to show multiple perspectives or players simultaneously." ;
  rdfs:seeAlso <http://dbpedia.org/resource/Split_screen_(computing)> ;
  schema:url <https://store.steampowered.com/tags/en/Split%20Screen/> .

steam:Stylized a owl:Class, steam:VisualsAndViewpoint ;
  rdfs:label "Stylized" ;
  rdfs:comment "Stylized refers to a visual style that distorts or exaggerates certain elements for expressive or artistic effect." ;
  schema:url <https://store.steampowered.com/tags/en/Stylized/> .

steam:TextBased a owl:Class, steam:VisualsAndViewpoint ;
  rdfs:label "Text-Based" ;
  rdfs:comment "Text-Based refers to a style of game where the visuals are primarily composed of text. These games often rely heavily on narrative and allow for extensive player imagination." ;
  rdfs:seeAlso <http://dbpedia.org/resource/Text-based_game> ;
  schema:url <https://store.steampowered.com/tags/en/Text-Based/> .

steam:ThirdPerson a owl:Class, steam:VisualsAndViewpoint ;
  rdfs:label "Third Person" ;
  rdfs:comment "Third Person refers to a perspective in which the player views the game world from over the shoulder or behind the main character." ;
  schema:url <https://store.steampowered.com/tags/en/Third%20Person/> .

steam:TopDown a owl:Class, steam:VisualsAndViewpoint ;
  rdfs:label "Top-Down" ;
  rdfs:comment "Top-Down refers to a perspective in which the player views the game world from above, often used in strategy and simulation games." ;
  rdfs:seeAlso <http://dbpedia.org/resource/Top-down_perspective> ;
  schema:url <https://store.steampowered.com/tags/en/Top-Down/> .

steam:Voxel a owl:Class, steam:VisualsAndViewpoint ;
  rdfs:label "Voxel" ;
  rdfs:comment "Voxel refers to a visual style that uses volumetric pixels (voxels) to create the game world. This style is often associated with 3D games that have a blocky or cubic aesthetic." ;
  rdfs:seeAlso <http://dbpedia.org/resource/Voxel> ;
  schema:url <https://store.steampowered.com/tags/en/Voxel/> .

steam:VR a owl:Class, steam:VisualsAndViewpoint ;
  rdfs:label "VR" ;
  rdfs:comment "VR, or Virtual Reality, refers to a technology that allows players to experience a game in a three-dimensional, interactive environment." ;
  rdfs:seeAlso <http://dbpedia.org/resource/Virtual_reality> ;
  schema:url <https://store.steampowered.com/tags/en/VR/> .

# Themes and Moods tags

steam:1980s a owl:Class, steam:ThemesAndMoods ;
  rdfs:label "1980s" ;
  rdfs:comment "The 1980s tag encapsulates the vibrant pop culture, technological optimism, and distinctive aesthetics of this decade. Games with this tag might feature neon colors, synth music, or references to iconic 80s events and personalities." ;
  rdfs:seeAlso <http://dbpedia.org/resource/1980s> ;
  schema:url <https://store.steampowered.com/tags/en/1980s/> .

steam:1990s a owl:Class, steam:ThemesAndMoods ;
  rdfs:label "1990s" ;
  rdfs:comment "The 1990s tag captures the spirit of this transformative decade, marked by the rise of the internet, grunge music, and a distinctive blend of optimism and cynicism. Games with this tag might feature early internet culture, iconic 90s fashion, or the decade's unique blend of music and art." ;
  rdfs:seeAlso <http://dbpedia.org/resource/1990s> ;
  schema:url <https://store.steampowered.com/tags/en/1990s/> .

steam:Agriculture a owl:Class, steam:ThemesAndMoods ;
  rdfs:label "Agriculture" ;
  rdfs:comment "The Agriculture tag is used for games that allow players to cultivate and manage their own farms, gardens, or vineyards. These games often emphasize patience, planning, and a connection with the land." ;
  rdfs:seeAlso <http://dbpedia.org/resource/Agriculture> ;
  schema:url <https://store.steampowered.com/tags/en/Agriculture/> .

steam:Aliens a owl:Class, steam:ThemesAndMoods ;
  rdfs:label "Aliens" ;
  rdfs:comment "The Aliens tag is used for games that feature extraterrestrial life. These games often explore themes of exploration, discovery, and sometimes conflict with unknown life forms." ;
  rdfs:seeAlso <http://dbpedia.org/resource/Extraterrestrial_life> ;
  schema:url <https://store.steampowered.com/tags/en/Aliens/> .

steam:AlternateHistory a owl:Class, steam:ThemesAndMoods ;
  rdfs:label "Alternate History" ;
  rdfs:comment "The Alternate History tag is used for games that re-imagine history. These games explore 'what if' scenarios, providing a unique twist on historical events or periods." ;
  rdfs:seeAlso <http://dbpedia.org/resource/Alternate_history> ;
  schema:url <https://store.steampowered.com/tags/en/Alternate%20History/> .

steam:America a owl:Class, steam:ThemesAndMoods ;
  rdfs:label "America" ;
  rdfs:comment "The America tag is used for games that explore aspects of American life, history, or culture. These games might feature iconic American landscapes, historical events, or cultural touchstones." ;
  rdfs:seeAlso <http://dbpedia.org/resource/United_States> ;
  schema:url <https://store.steampowered.com/tags/en/America/> .

steam:Atmospheric a owl:Class, steam:ThemesAndMoods ;
  rdfs:label "Atmospheric" ;
  rdfs:comment "The Atmospheric tag is used for games that place a strong emphasis on creating a specific mood or feeling. These games often use detailed environments, sound design, and visual aesthetics to draw players into their world." ;
  schema:url <https://store.steampowered.com/tags/en/Atmospheric/> .

steam:Assassin a owl:Class, steam:ThemesAndMoods ;
  rdfs:label "Assassin" ;
  rdfs:comment "The Assassin tag is used for games that place the player in the role of an assassin. These games often involve stealth, strategy, and sometimes moral ambiguity as players navigate the shadowy world of their profession." ;
  schema:url <https://store.steampowered.com/tags/en/Assassin/> .

steam:Bikes a owl:Class, steam:ThemesAndMoods ;
  rdfs:label "Bikes" ;
  rdfs:comment "The Bikes tag is used for games that feature bicycles or motorcycles as a significant element. These games might involve racing, stunts, or simply the joy of exploring on two wheels." ;
  schema:url <https://store.steampowered.com/tags/en/Bikes/> .

steam:Capitalism a owl:Class, steam:ThemesAndMoods ;
  rdfs:label "Capitalism" ;
  rdfs:comment "The Capitalism tag is used for games that explore themes of free-market economics. These games might involve running a business, trading stocks, or navigating the complex world of finance." ;
  rdfs:seeAlso <http://dbpedia.org/resource/Capitalism> ;
  schema:url <https://store.steampowered.com/tags/en/Capitalism/> .

steam:Cats a owl:Class, steam:ThemesAndMoods ;
  rdfs:label "Cats" ;
  rdfs:comment "The Cats tag is used for games that feature cats as a significant element. These games might involve caring for cats, playing as a cat, or simply feature cats as part of the game's world." ;
  rdfs:seeAlso <http://dbpedia.org/resource/Cat> ;
  schema:url <https://store.steampowered.com/tags/en/Cats/> .

steam:ColdWar a owl:Class, steam:ThemesAndMoods ;
  rdfs:label "Cold War" ;
  rdfs:comment "The Cold War tag is used for games that explore the tense geopolitical period from 1947 to 1991. These games might involve espionage, nuclear brinkmanship, or the ideological clash between capitalism and communism." ;
  rdfs:seeAlso <http://dbpedia.org/resource/Cold_War> ;
  schema:url <https://store.steampowered.com/tags/en/Cold%20War/> .

steam:ComicBook a owl:Class, steam:ThemesAndMoods .

steam:Conspiracy a owl:Class, steam:ThemesAndMoods ;
  rdfs:label "Conspiracy" ;
  rdfs:comment "The Conspiracy tag is used for games that delve into the world of secret plots and hidden agendas. These games might involve unraveling complex mysteries, navigating shadowy organizations, or uncovering hidden truths." ;
  rdfs:seeAlso <http://dbpedia.org/resource/Conspiracy_theory> ;
  schema:url <https://store.steampowered.com/tags/en/Conspiracy/> .

steam:Crime a owl:Class, steam:ThemesAndMoods ;
  rdfs:label "Crime" ;
  rdfs:comment "The Crime tag is used for games that involve the world of crime as a significant element. These games might involve playing as a criminal, solving crimes, or exploring the impact of crime on individuals and societies." ;
  rdfs:seeAlso <http://dbpedia.org/resource/Crime> ;
  schema:url <https://store.steampowered.com/tags/en/Crime/> .

steam:Cyberpunk a owl:Class, steam:ThemesAndMoods ;
  rdfs:label "Cyberpunk" ;
  rdfs:comment "The Cyberpunk tag is used for games that explore themes of a dystopian future dominated by advanced technology, corporate power, and social inequality. These games often feature neon-lit cityscapes, rogue AI, and anti-hero protagonists." ;
  rdfs:seeAlso <http://dbpedia.org/resource/Cyberpunk> ;
  schema:url <https://store.steampowered.com/tags/en/Cyberpunk/> .

steam:Dark a owl:Class, steam:ThemesAndMoods ;
  rdfs:label "Dark" ;
  rdfs:comment "The Dark tag is used for games that feature a dark, often unsettling atmosphere. These games might involve horror elements, mature themes, or a sense of dread and unease." ;
  schema:url <https://store.steampowered.com/tags/en/Dark/> .

steam:DarkFantasy a owl:Class, steam:ThemesAndMoods ;
  rdfs:label "Dark Fantasy" ;
  rdfs:comment "The Dark Fantasy tag is used for games that blend the fantastical elements of fantasy with darker, more horrifying themes. These games often feature grim settings, morally ambiguous characters, and a sense of impending doom." ;
  rdfs:seeAlso <http://dbpedia.org/resource/Dark_fantasy> ;
  schema:url <https://store.steampowered.com/tags/en/Dark%20Fantasy/> .

steam:Demons a owl:Class, steam:ThemesAndMoods ;
  rdfs:label "Demons" ;
  rdfs:comment "The Demons tag is used for games that feature demons and might involve battling demons, playing as a demon, or exploring a world where demons exist." ;
  rdfs:seeAlso <http://dbpedia.org/resource/Demon> ;
  schema:url <https://store.steampowered.com/tags/en/Demons/> .

steam:Destruction a owl:Class, steam:ThemesAndMoods ;
  rdfs:label "Destruction" ;
  rdfs:comment "The Destruction tag is used for games that might involve destroying environments, buildings, or other structures as part of the gameplay." ;
  rdfs:seeAlso <http://dbpedia.org/resource/Destruction> ;
  schema:url <https://store.steampowered.com/tags/en/Destruction/> .

steam:Detective a owl:Class, steam:ThemesAndMoods ;
  rdfs:label "Detective" ;
  rdfs:comment "The Detective tag is used for games that involve detective work and may involve solving mysteries, investigating crimes, or playing as a detective character." ;
  rdfs:seeAlso <http://dbpedia.org/resource/Detective> ;
  schema:url <https://store.steampowered.com/tags/en/Detective/> .

steam:Dinosaurs a owl:Class, steam:ThemesAndMoods ;
  rdfs:label "Dinosaurs" ;
  rdfs:comment "The Dinosaurs tag is used for games that feature dinosaurs and may involve interacting with dinosaurs, playing as a dinosaur, or exploring a world where dinosaurs exist." ;
  rdfs:seeAlso <http://dbpedia.org/resource/Dinosaur> ;
  schema:url <https://store.steampowered.com/tags/en/Dinosaurs/> .

steam:Diplomacy a steam:ThemesAndMoods .

steam:Dog a owl:Class, steam:ThemesAndMoods ;
  rdfs:label "Dog" ;
  rdfs:comment "The Dog tag is used for games that feature dogs. These games might involve caring for dogs, playing as a dog, or simply feature dogs as part of the game's world." ;
  rdfs:seeAlso <http://dbpedia.org/resource/Dog> ;
  schema:url <https://store.steampowered.com/tags/en/Dog/> .

steam:Dragons a owl:Class, steam:ThemesAndMoods ;
  rdfs:label "Dragons" ;
  rdfs:comment "The Dragons tag is used for games that may involve battling dragons, playing as a dragon, or exploring a world where dragons exist." ;
  rdfs:seeAlso <http://dbpedia.org/resource/Dragon> ;
  schema:url <https://store.steampowered.com/tags/en/Dragons/> .

steam:DynamicNarration a owl:Class, steam:ThemesAndMoods ;
  rdfs:label "Dynamic Narration" ;
  rdfs:comment "The Dynamic Narration tag is used for games that feature a narrative that changes based on player actions. These games often offer a high degree of player agency and multiple branching story paths." ;
  schema:url <https://store.steampowered.com/tags/en/Dynamic%20Narration/> .

steam:Economy a owl:Class, steam:ThemesAndMoods ;
  rdfs:label "Economy" ;
  rdfs:comment "The Economy tag is used for games that involve economic systems. These games might involve trading, resource management, or running a business." ;
  rdfs:seeAlso <http://dbpedia.org/resource/Economy> ;
  schema:url <https://store.steampowered.com/tags/en/Economy/> .

steam:Education a owl:Class, steam:ThemesAndMoods .

steam:Faith a owl:Class, steam:ThemesAndMoods ;
  rdfs:label "Faith" ;
  rdfs:comment "The Faith tag is used for games that explore themes of faith, religion, or spirituality. These games might involve exploring religious beliefs, engaging with spiritual practices, or navigating the complexities of faith." ;
  rdfs:seeAlso <http://dbpedia.org/resource/Faith> ;
  schema:url <https://store.steampowered.com/tags/en/Faith/> .

steam:FamilyFriendly a owl:Class, steam:ThemesAndMoods ;
  rdfs:label "Family Friendly" ;
  rdfs:comment "The Family Friendly tag is used for games that are suitable for players of all ages. These games often avoid explicit content, focus on positive themes, and are designed to be accessible and enjoyable for a wide audience." ;
  schema:url <https://store.steampowered.com/tags/en/Family%20Friendly/> .

steam:Fantasy a owl:Class, steam:ThemesAndMoods ;
  rdfs:label "Fantasy" ;
  rdfs:comment "The Fantasy tag is used for games that feature elements of fantasy, such as magic, mythical creatures, or fantastical settings. These games often involve quests, epic narratives, and exploration of magical worlds." ;
  rdfs:seeAlso <http://dbpedia.org/resource/Fantasy> ;
  schema:url <https://store.steampowered.com/tags/en/Fantasy/> .

steam:Foreign a owl:Class, steam:ThemesAndMoods ;
  rdfs:label "Foreign" ;
  rdfs:comment "The Foreign tag is used for games that originate from or are set in countries outside of the player's own. These games often offer insights into different cultures, languages, and perspectives." ;
  schema:url <https://store.steampowered.com/tags/en/Foreign/> .

steam:Futuristic a owl:Class, steam:ThemesAndMoods ;
  rdfs:label "Futuristic" ;
  rdfs:comment "The Futuristic tag is used for games that are set in or draw inspiration from visions of the future. These games often feature advanced technology, futuristic settings, and themes of exploration and innovation." ;
  rdfs:seeAlso <http://dbpedia.org/resource/Future> ;
  schema:url <https://store.steampowered.com/tags/en/Futuristic/> .

steam:Gambling a owl:Class, steam:ThemesAndMoods ;
  rdfs:label "Gambling" ;
  rdfs:comment "The Gambling tag is used for games that involve playing casino games, betting on outcomes, or other forms of wagering." ;
  rdfs:seeAlso <http://dbpedia.org/resource/Gambling> ;
  schema:url <https://store.steampowered.com/tags/en/Gambling/> .

steam:GameDevelopment a owl:Class, steam:ThemesAndMoods ;
  rdfs:label "Game Development" ;
  rdfs:comment "The Game Development tag is used for games that might involve creating your own games, managing a game development studio, or exploring the process of game development." ;
  rdfs:seeAlso <http://dbpedia.org/resource/Video_game_development> ;
  schema:url <https://store.steampowered.com/tags/en/Game%20Development/> .

steam:Gothic a owl:Class, steam:ThemesAndMoods ;
  rdfs:label "Gothic" ;
  rdfs:comment "The Gothic tag is used for games that feature gothic themes or aesthetics. These games might involve dark and atmospheric settings, supernatural elements, or a focus on horror and mystery." ;
  rdfs:seeAlso <http://dbpedia.org/resource/Gothic_fiction> ;
  schema:url <https://store.steampowered.com/tags/en/Gothic/> .

steam:Heist a steam:ThemesAndMoods .

steam:Historical a owl:Class, steam:ThemesAndMoods ;
  rdfs:label "Historical" ;
  rdfs:comment "The Historical tag is used for games that are set in or draw inspiration from real historical periods. These games often involve exploring historical events, interacting with historical figures, or recreating historical settings." ;
  rdfs:seeAlso <http://dbpedia.org/resource/History> ;
  schema:url <https://store.steampowered.com/tags/en/Historical/> .

steam:Horses a owl:Class, steam:ThemesAndMoods ;
  rdfs:label "Horses" ;
  rdfs:comment "The Horses tag is used for games that feature horses. These games might involve riding horses, caring for horses, or exploring a world where horses play a significant role." ;
  rdfs:seeAlso <http://dbpedia.org/resource/Horse> ;
  schema:url <https://store.steampowered.com/tags/en/Horses/> .

steam:Illuminati a owl:Class, steam:ThemesAndMoods ;
  rdfs:label "Illuminati" ;
  rdfs:comment "The Illuminati tag is used for games that involve the Illuminati or similar secret societies as a significant element. These games might involve uncovering conspiracies, battling secret societies, or exploring the influence of all-powerful organizations." ;
  rdfs:seeAlso <http://dbpedia.org/resource/Illuminati> ;
  schema:url <https://store.steampowered.com/tags/en/Illuminati/> .

steam:Investigation a owl:Class, steam:ThemesAndMoods .

steam:Jet a owl:Class, steam:ThemesAndMoods ;
  rdfs:label "Jet" ;
  rdfs:comment "The Jet tag is used for games that feature jets or jet-powered vehicles. These games might involve flying jets, participating in jet combat, or exploring a world where jets play a significant role." ;
  rdfs:seeAlso <http://dbpedia.org/resource/Jet_aircraft> ;
  schema:url <https://store.steampowered.com/tags/en/Jet/> .

steam:Lemmings a owl:Class, steam:ThemesAndMoods ;
  rdfs:label "Lemmings" ;
  rdfs:comment "The Lemmings tag is used for games that feature gameplay mechanics similar to the classic game Lemmings. These games often involve guiding a group of characters through a series of obstacles to reach a goal." ;
  rdfs:seeAlso <http://dbpedia.org/resource/Lemmings_(video_game)> ;
  schema:url <https://store.steampowered.com/tags/en/Lemmings/> .

steam:LGBTQPlus a owl:Class, steam:ThemesAndMoods ;
  rdfs:label "LGBTQ+" ;
  rdfs:comment "The LGBTQ+ tag is used for games that feature LGBTQ+ themes or characters as a significant element. These games might involve exploring LGBTQ+ identities, relationships, or issues, or feature LGBTQ+ characters in prominent roles." ;
  rdfs:seeAlso <http://dbpedia.org/resource/LGBT> ;
  schema:url <https://store.steampowered.com/tags/en/LGBTQ%2B/> .

steam:Logic a owl:Class, steam:ThemesAndMoods ;
  rdfs:label "Logic" ;
  rdfs:comment "The Logic tag is used for games that involve logic puzzles. These games might involve solving puzzles, deducing solutions, or applying logical reasoning to overcome challenges." ;
  rdfs:seeAlso <http://dbpedia.org/resource/Logic> ;
  schema:url <https://store.steampowered.com/tags/en/Logic/> .

steam:Loot a owl:Class, steam:ThemesAndMoods ;
  rdfs:label "Loot" ;
  rdfs:comment "The Loot tag is used for games that feature loot or item collection as a significant element. These games might involve finding and collecting items and upgrading equipment." ;
  rdfs:seeAlso <http://dbpedia.org/resource/Loot> ;
  schema:url <https://store.steampowered.com/tags/en/Loot/> .

steam:Lovecraftian a owl:Class, steam:ThemesAndMoods ;
  rdfs:label "Lovecraftian" ;
  rdfs:comment "The Lovecraftian tag is used for games that feature themes, settings, or elements inspired by the works of H.P. Lovecraft. These games often involve cosmic horror, ancient gods, or a sense of dread and the unknown." ;
  rdfs:seeAlso <http://dbpedia.org/resource/Lovecraftian_horror> ;
  schema:url <https://store.steampowered.com/tags/en/Lovecraftian/> .

steam:Magic a owl:Class, steam:ThemesAndMoods ;
  rdfs:label "Magic" ;
  rdfs:comment "The Magic tag is used for games that feature magic or magical elements as a significant aspect. These games might involve casting spells, exploring magical worlds, or interacting with magical creatures." ;
  rdfs:seeAlso <http://dbpedia.org/resource/Magic_(supernatural)> ;
  schema:url <https://store.steampowered.com/tags/en/Magic/> .

steam:Management a steam:ThemesAndMoods .

steam:Mars a owl:Class, steam:ThemesAndMoods ;
  rdfs:label "Mars" ;
  rdfs:comment "The Mars tag is used for games that feature Mars or Martian elements. These games might involve exploring Mars, interacting with Martian life, or surviving in a Martian environment." ;
  rdfs:seeAlso <http://dbpedia.org/resource/Mars> ;
  schema:url <https://store.steampowered.com/tags/en/Mars/> .

steam:Mechs a owl:Class, steam:ThemesAndMoods ;
  rdfs:label "Mechs" ;
  rdfs:comment "The Mechs tag is used for games that feature mechs or mech combat. These games might involve piloting mechs, battling with mechs, or exploring a world where mechs play a significant role." ;
  rdfs:seeAlso <http://dbpedia.org/resource/Mecha> ;
  schema:url <https://store.steampowered.com/tags/en/Mechs/> .

steam:Medieval a owl:Class, steam:ThemesAndMoods ;
  rdfs:label "Medieval" ;
  rdfs:comment "The Medieval tag is used for games that are set in or draw inspiration from the medieval period. These games often involve exploring medieval settings, interacting with medieval characters, or recreating medieval life." ;
  schema:url <https://store.steampowered.com/tags/en/Medieval/> .

steam:Memes a owl:Class, steam:ThemesAndMoods ;
  rdfs:label "Memes" ;
  rdfs:comment "The Memes tag is used for games that feature memes or meme culture." ;
  rdfs:seeAlso <http://dbpedia.org/resource/Internet_meme> ;
  schema:url <https://store.steampowered.com/tags/en/Memes/> .

steam:Military a owl:Class, steam:ThemesAndMoods ;
  rdfs:label "Military" ;
  rdfs:comment "The Military tag is used for games that may involve participating in military operations, exploring military history, or interacting with military equipment and personnel." ;
  rdfs:seeAlso <http://dbpedia.org/resource/Military> ;
  schema:url <https://store.steampowered.com/tags/en/Military/> .

steam:Modern a owl:Class, steam:ThemesAndMoods ;
  rdfs:label "Modern" ;
  rdfs:comment "The Modern tag is used for games that are set in or draw inspiration from the modern period or dealing with modern issues and themes." ;
  schema:url <https://store.steampowered.com/tags/en/Modern/> .

steam:Motorbike a owl:Class, steam:ThemesAndMoods ;
  rdfs:label "Motorbike" ;
  rdfs:comment "The Motorbike tag is used for games that feature motorbikes or motorbike racing." ;
  rdfs:seeAlso <http://dbpedia.org/resource/Motorcycle> ;
  schema:url <https://store.steampowered.com/tags/en/Motorbike/> .

steam:Mystery a owl:Class, steam:ThemesAndMoods ;
  rdfs:label "Mystery" ;
  rdfs:comment "The Mystery tag is used for games that feature mystery or suspense. These games might involve solving mysteries and uncovering secrets." ;
  rdfs:seeAlso <http://dbpedia.org/resource/Mystery_fiction> ;
  schema:url <https://store.steampowered.com/tags/en/Mystery/> .

steam:Mythology a owl:Class, steam:ThemesAndMoods ;
  rdfs:label "Mythology" ;
  rdfs:comment "The Mythology tag is used for games that feature mythology and may involve exploring mythological worlds, interacting with mythological creatures, or delving into mythological lore." ;
  rdfs:seeAlso <http://dbpedia.org/resource/Mythology> ;
  schema:url <https://store.steampowered.com/tags/en/Mythology/> .

steam:Nature a owl:Class, steam:ThemesAndMoods ;
  rdfs:label "Nature" ;
  rdfs:comment "The Nature tag is used for games that feature nature or natural environments and may involve exploring natural landscapes and interacting with wildlife." ;
  rdfs:seeAlso <http://dbpedia.org/resource/Nature> ;
  schema:url <https://store.steampowered.com/tags/en/Nature/> .

steam:Naval a owl:Class, steam:ThemesAndMoods ;
  rdfs:label "Naval" ;
  rdfs:comment "The Naval tag is used for games that feature naval or maritime elements as a significant aspect. These games might involve commanding naval vessels, engaging in naval combat, or exploring maritime environments." ;
  schema:url <https://store.steampowered.com/tags/en/Naval/> .

steam:Ninja a owl:Class, steam:ThemesAndMoods ;
  rdfs:label "Ninja" ;
  rdfs:comment "The Ninja tag is used for games that feature ninjas or ninja-themed elements as a significant aspect. These games might involve playing as a ninja, using ninja tactics, or exploring a world influenced by ninja culture." ;
  rdfs:seeAlso <http://dbpedia.org/resource/Ninja> ;
  schema:url <https://store.steampowered.com/tags/en/Ninja/> .

steam:Offroad a owl:Class, steam:ThemesAndMoods ;
  rdfs:label "Offroad" ;
  rdfs:comment "The Offroad tag is used for games that might involve driving offroad vehicles, navigating challenging terrains, or exploring remote environments." ;
  rdfs:seeAlso <http://dbpedia.org/resource/Off-roading> ;
  schema:url <https://store.steampowered.com/tags/en/Offroad/> .

steam:OldSchool a owl:Class, steam:ThemesAndMoods ;
  rdfs:label "Old School" ;
  rdfs:comment "The Old School tag is used for games that feature old school or retro elements as a significant aspect. These games might involve classic gameplay mechanics, retro graphics, or nostalgic themes." ;
  rdfs:seeAlso <http://dbpedia.org/resource/Retrogaming> ;
  schema:url <https://store.steampowered.com/tags/en/Old%20School/> .

steam:Otome a owl:Class, steam:ThemesAndMoods ;
  rdfs:label "Otome" ;
  rdfs:comment "The Otome tag is used for games that are designed with the typical preferences of women in mind, and one of the main goals, besides the plot goal, is to develop a romantic relationship between the female player character and one of several male or female characters. This genre is most established in Japan, and is mostly made up of visual novels and simulation games." ;
  rdfs:seeAlso <http://dbpedia.org/resource/Otome_game> ;
  schema:url <https://store.steampowered.com/tags/en/Otome/> .

steam:Parkour a owl:Class, steam:ThemesAndMoods ;
  rdfs:label "Parkour" ;
  rdfs:comment "The Parkour tag is used for games that feature parkour or free-running elements as a significant aspect." ;
  rdfs:seeAlso <http://dbpedia.org/resource/Parkour> ;
  schema:url <https://store.steampowered.com/tags/en/Parkour/> .

steam:Philosophical a owl:Class, steam:ThemesAndMoods ;
  rdfs:label "Philosophical" ;
  rdfs:comment "The Philosophical tag is used for games that feature philosophical themes or thought-provoking elements." ;
  rdfs:seeAlso <http://dbpedia.org/resource/Philosophy> ;
  schema:url <https://store.steampowered.com/tags/en/Philosophical/> .

steam:Pirates a owl:Class, steam:ThemesAndMoods ;
  rdfs:label "Pirates" ;
  rdfs:comment "The Pirates tag is used for games that feature pirates or piracy elements that might involve sailing pirate ships, engaging in pirate combat, or exploring a world influenced by pirate culture." ;
  rdfs:seeAlso <http://dbpedia.org/resource/Piracy> ;
  schema:url <https://store.steampowered.com/tags/en/Pirates/> .

steam:Political a owl:Class, steam:ThemesAndMoods ;
  rdfs:label "Political" ;
  rdfs:comment "The Political tag is often associated with games that deal with political science concepts. This could include the theoretical analysis of political systems, their origins, underlying values, and goals." ;
  rdfs:seeAlso <http://dbpedia.org/resource/Politics> ;
  schema:url <https://store.steampowered.com/tags/en/Political/> .

steam:Politics a owl:Class, steam:ThemesAndMoods ;
  rdfs:label "Politics" ;
  rdfs:comment "The Politics tag generally refers to games that involve activities related to governance or influencing the way a country or organization is governed. This could include decision-making processes, implementation of laws and norms within a game's universe, or strategies aimed at improving the lives of the game's characters." ;
  rdfs:seeAlso <http://dbpedia.org/resource/Politics> ;
  schema:url <https://store.steampowered.com/tags/en/Politics/> .

steam:Pool a owl:Class, steam:ThemesAndMoods ;
  rdfs:label "Pool" ;
  rdfs:comment "The Pool tag is used for games that feature pool or billiards elements." ;
  rdfs:seeAlso <http://dbpedia.org/resource/Cue_sports> ;
  schema:url <https://store.steampowered.com/tags/en/Pool/> .

steam:PostApocalyptic a owl:Class, steam:ThemesAndMoods ;
  rdfs:label "Post-apocalyptic" ;
  rdfs:comment "The Post-apocalyptic tag is used for games that feature post-apocalyptic themes." ;
  rdfs:seeAlso <http://dbpedia.org/resource/Post-apocalyptic> ;
  schema:url <https://store.steampowered.com/tags/en/Post-apocalyptic/> .

steam:Programming a owl:Class, steam:ThemesAndMoods .

steam:Retro a owl:Class, steam:ThemesAndMoods ;
  rdfs:label "Retro" ;
  rdfs:comment "The Retro tag is used for games that feature retro or vintage elements as a significant aspect. These games might involve retro graphics, vintage soundtracks, or gameplay mechanics reminiscent of older games." ;
  rdfs:seeAlso <http://dbpedia.org/resource/Retrogaming> ;
  schema:url <https://store.steampowered.com/tags/en/Retro/> .

steam:Robots a owl:Class, steam:ThemesAndMoods ;
  rdfs:label "Robots" ;
  rdfs:comment "The Robots tag is used for games that feature robots or robotics elements." ;
  rdfs:seeAlso <http://dbpedia.org/resource/Robot> ;
  schema:url <https://store.steampowered.com/tags/en/Robots/> .

steam:Romance a owl:Class, steam:ThemesAndMoods ;
  rdfs:label "Romance" ;
  rdfs:comment "The Romance tag is used for games that feature romance or romantic elements." ;
  rdfs:seeAlso <http://dbpedia.org/resource/Romance_(love)> ;
  schema:url <https://store.steampowered.com/tags/en/Romance/> .

steam:Rome a owl:Class, steam:ThemesAndMoods ;
  rdfs:label "Rome" ;
  rdfs:comment "The Rome tag is used for games that feature Rome or Roman elements and may involve Roman history or Roman mythology." ;
  rdfs:seeAlso <http://dbpedia.org/resource/Ancient_Rome> ;
  schema:url <https://store.steampowered.com/tags/en/Rome/> .

steam:Satire a owl:Class, steam:ThemesAndMoods ;
  rdfs:label "Satire" ;
  rdfs:comment "The Satire tag is used for games that feature satirical humor, satirical commentary, or satirical themes." ;
  rdfs:seeAlso <http://dbpedia.org/resource/Satire> ;
  schema:url <https://store.steampowered.com/tags/en/Satire/> .

steam:Science a owl:Class, steam:ThemesAndMoods ;
  rdfs:label "Science" ;
  rdfs:comment "The Science tag is used for games may involve scientific concepts, scientific exploration, or settings based on scientific theories." ;
  rdfs:seeAlso <http://dbpedia.org/resource/Science> ;
  schema:url <https://store.steampowered.com/tags/en/Science/> .

steam:SciFi a owl:Class, steam:ThemesAndMoods ;
  rdfs:label "Sci-fi" ;
  rdfs:comment "The Sci-fi tag is used for games that feature science fiction or sci-fi elements as a significant aspect. These games might involve futuristic technology, alien worlds, or themes common in science fiction." ;
  rdfs:seeAlso <http://dbpedia.org/resource/Science_fiction> ;
  schema:url <https://store.steampowered.com/tags/en/Sci-fi/> .

steam:Sniper a owl:Class, steam:ThemesAndMoods ;
  rdfs:label "Sniper" ;
  rdfs:comment "The Sniper tag is used for games that feature sniper or sniping elements. These games might involve sniper rifles, sniper missions, or gameplay mechanics focused on precision and patience." ;
  rdfs:seeAlso <http://dbpedia.org/resource/Sniper> ;
  schema:url <https://store.steampowered.com/tags/en/Sniper/> .

steam:Snow a owl:Class, steam:ThemesAndMoods ;
  rdfs:label "Snow" ;
  rdfs:comment "The Snow tag is used for games that feature snow or snowy environments. These games might involve snow landscapes or snow sports." ;
  rdfs:seeAlso <http://dbpedia.org/resource/Snow> ;
  schema:url <https://store.steampowered.com/tags/en/Snow/> .

steam:Space a owl:Class, steam:ThemesAndMoods ;
  rdfs:label "Space" ;
  rdfs:comment "The Space tag is used for games that feature space or space exploration as a significant aspect. These games might involve space travel, alien planets, or settings in outer space." ;
  rdfs:seeAlso <http://dbpedia.org/resource/Outer_space> ;
  schema:url <https://store.steampowered.com/tags/en/Space/> .

steam:Stealth a steam:ThemesAndMoods .

steam:Steampunk a owl:Class, steam:ThemesAndMoods ;
  rdfs:label "Steampunk" ;
  rdfs:comment "A subgenre of science fiction characterized by the setting of an alternate history—typically Victorian era or American 'Wild West'—where steam power remains a primary technology. It combines retro futuristic technology and aesthetics, often inspired by 19th-century industrial steam-powered machinery." ;
  rdfs:seeAlso <http://dbpedia.org/resource/Steampunk> ;
  schema:url <https://store.steampowered.com/tags/en/Steampunk/> .

steam:Submarine a owl:Class, steam:ThemesAndMoods ;
  rdfs:label "Submarine" ;
  rdfs:comment "The Submarine tag is used for games that feature submarines or submarine-based gameplay." ;
  rdfs:seeAlso <http://dbpedia.org/resource/Submarine> ;
  schema:url <https://store.steampowered.com/tags/en/Submarine/> .

steam:Superhero a owl:Class, steam:ThemesAndMoods ;
  rdfs:label "Superhero" ;
  rdfs:comment "The Superhero tag is used for games that feature superhero themes." ;
  rdfs:seeAlso <http://dbpedia.org/resource/Superhero> ;
  schema:url <https://store.steampowered.com/tags/en/Superhero/> .

steam:Supernatural a owl:Class, steam:ThemesAndMoods ;
  rdfs:label "Supernatural" ;
  rdfs:comment "The Supernatural tag is used for games that feature supernatural themes." ;
  rdfs:seeAlso <http://dbpedia.org/resource/Supernatural> ;
  schema:url <https://store.steampowered.com/tags/en/Supernatural/> .

steam:Surreal a owl:Class, steam:ThemesAndMoods ;
  rdfs:label "Surreal" ;
  rdfs:comment "The Surreal tag is used for games that feature surreal or surrealistic elements as a significant aspect. These games might involve dream-like landscapes, bizarre characters, or gameplay mechanics that defy reality." ;
  rdfs:seeAlso <http://dbpedia.org/resource/Surrealism> ;
  schema:url <https://store.steampowered.com/tags/en/Surreal/> .

steam:Survival a owl:Class, steam:ThemesAndMoods .

steam:Swordplay a owl:Class, steam:ThemesAndMoods ;
  rdfs:label "Swordplay" ;
  rdfs:comment "The Swordplay tag is used for games that feature sword fights, historical fencing, or gameplay mechanics focused on swordplay." ;
  rdfs:seeAlso <http://dbpedia.org/resource/Swordsmanship> ;
  schema:url <https://store.steampowered.com/tags/en/Swordplay/> .

steam:Tactical a owl:Class, steam:ThemesAndMoods ;
  rdfs:label "Tactical" ;
  rdfs:comment "The Tactical tag is used for games that feature tactical or strategy-based gameplay as a significant aspect. These games might involve tactical combat, strategic planning, or gameplay mechanics focused on tactics." ;
  schema:url <https://store.steampowered.com/tags/en/Tactical/> .

steam:Tanks a owl:Class, steam:ThemesAndMoods ;
  rdfs:label "Tanks" ;
  rdfs:comment "The Tanks tag is used for games that feature tanks or tank-based combat." ;
  rdfs:seeAlso <http://dbpedia.org/resource/Tank> ;
  schema:url <https://store.steampowered.com/tags/en/Tanks/> .

steam:Thriller a owl:Class, steam:ThemesAndMoods ;
  rdfs:label "Thriller" ;
  rdfs:comment "The Thriller tag is used for games that feature suspenseful narratives, thrilling scenarios, or gameplay mechanics focused on creating tension." ;
  rdfs:seeAlso <http://dbpedia.org/resource/Thriller_(genre)> ;
  schema:url <https://store.steampowered.com/tags/en/Thriller/> .

steam:TimeTravel a owl:Class, steam:ThemesAndMoods ;
  rdfs:label "Time Travel" ;
  rdfs:comment "The Time Travel tag is used for games that feature traveling through time, changing history, or gameplay mechanics focused on time manipulation." ;
  rdfs:seeAlso <http://dbpedia.org/resource/Time_travel> ;
  schema:url <https://store.steampowered.com/tags/en/Time%20Travel/> .

steam:Trains a owl:Class, steam:ThemesAndMoods ;
  rdfs:label "Trains" ;
  rdfs:comment "The Trains tag is used for games that feature trains and might involve controlling a train, managing a railway, etc." ;
  rdfs:seeAlso <http://dbpedia.org/resource/Train> ;
  schema:url <https://store.steampowered.com/tags/en/Trains/> .

steam:Transhumanism a owl:Class, steam:ThemesAndMoods ;
  rdfs:label "Transhumanism" ;
  rdfs:comment "The Transhumanism tag is used for games that feature transhumanism and might involve cybernetic enhancements, artificial intelligence, or themes related to the post-human condition." ;
  rdfs:seeAlso <http://dbpedia.org/resource/Transhumanism> ;
  schema:url <https://store.steampowered.com/tags/en/Transhumanism/> .

steam:Transportation a owl:Class, steam:ThemesAndMoods ;
  rdfs:label "Transportation" ;
  rdfs:comment "The Transportation tag is used for games that feature managing a transport network, controlling various vehicles, or gameplay mechanics focused on transportation." ;
  rdfs:seeAlso <http://dbpedia.org/resource/Transport> ;
  schema:url <https://store.steampowered.com/tags/en/Transportation/> .

steam:Underground a owl:Class, steam:ThemesAndMoods ;
  rdfs:label "Underground" ;
  rdfs:comment "The Underground tag is used for games that feature underground environments and might involve exploration of caves, dungeons, or other subterranean settings." ;
  schema:url <https://store.steampowered.com/tags/en/Underground/> .

steam:Underwater a owl:Class, steam:ThemesAndMoods ;
  rdfs:label "Underwater" ;
  rdfs:comment "The Underwater tag is used for games that involve underwater exploration, marine life, or gameplay mechanics focused on underwater navigation." ;
  rdfs:seeAlso <http://dbpedia.org/resource/Underwater> ;
  schema:url <https://store.steampowered.com/tags/en/Underwater/> .

steam:Vampire a owl:Class, steam:ThemesAndMoods ;
  rdfs:label "Vampire" ;
  rdfs:comment "The Vampire tag is used for games that feature vampire characters, vampire lore, or gameplay mechanics focused on vampiric abilities." ;
  rdfs:seeAlso <http://dbpedia.org/resource/Vampire> ;
  schema:url <https://store.steampowered.com/tags/en/Vampire/> .

steam:War a owl:Class, steam:ThemesAndMoods ;
  rdfs:label "War" ;
  rdfs:comment "The War tag is used for games that feature war or war themes." ;
  rdfs:seeAlso <http://dbpedia.org/resource/War> ;
  schema:url <https://store.steampowered.com/tags/en/War/> .

steam:Werewolves a owl:Class, steam:ThemesAndMoods ;
  rdfs:label "Werewolves" ;
  rdfs:comment "The Werewolves tag is used for games that feature werewolf characters, werewolf lore, or gameplay mechanics focused on lycanthropic abilities." ;
  rdfs:seeAlso <http://dbpedia.org/resource/Werewolf> ;
  schema:url <https://store.steampowered.com/tags/en/Werewolves/> .

steam:Western a owl:Class, steam:ThemesAndMoods ;
  rdfs:label "Western" ;
  rdfs:comment "The Western tag is used for games that feature Western or Wild West themes." ;
  rdfs:seeAlso <http://dbpedia.org/resource/Western_(genre)> ;
  schema:url <https://store.steampowered.com/tags/en/Western/> .

steam:WorldWarI a owl:Class, steam:ThemesAndMoods ;
  rdfs:label "World War I" ;
  rdfs:comment "The World War I tag is used for games that feature World War I historical events, WWI era settings, or gameplay mechanics focused on the WWI period." ;
  rdfs:seeAlso <http://dbpedia.org/resource/World_War_I> ;
  schema:url <https://store.steampowered.com/tags/en/World%20War%20I/> .

steam:WorldWarII a owl:Class, steam:ThemesAndMoods ;
  rdfs:label "World War II" ;
  rdfs:comment "The World War II tag is used for games that feature World War II historical events, WWII era settings, or gameplay mechanics focused on the WWII period." ;
  rdfs:seeAlso <http://dbpedia.org/resource/World_War_II> ;
  schema:url <https://store.steampowered.com/tags/en/World%20War%20II/> .

# Features tags

steam:6DOF a owl:Class, steam:Features ;
  rdfs:label "6DOF" ;
  rdfs:comment "6DOF (Six Degrees of Freedom) is a feature that allows full 3D spatial movement and rotation. This includes the ability to move forward/backward, up/down, left/right and to rotate along three perpendicular axes." ;
  rdfs:seeAlso <http://dbpedia.org/resource/Six_degrees_of_freedom> ;
  schema:url <https://store.steampowered.com/tags/en/6DOF/> .

steam:Archery a owl:Class, steam:Features ;
  rdfs:label "Archery" ;
  rdfs:comment "Archery is a feature that involves the use of bows and arrows as a primary mechanic. It often requires precision and timing, and can be used in combat, hunting, or sport scenarios within the game." ;
  rdfs:seeAlso <http://dbpedia.org/resource/Archery> ;
  schema:url <https://store.steampowered.com/tags/en/Archery/> .

steam:ArtificialIntelligence a owl:Class, steam:Features ;
  rdfs:label "Artificial Intelligence" ;
  rdfs:comment "Artificial Intelligence is a feature that involves the use of AI-controlled characters or systems. These can range from enemy combatants to friendly NPCs, and their behavior can significantly impact the gameplay experience." ;
  rdfs:seeAlso <http://dbpedia.org/resource/Artificial_intelligence> ;
  schema:url <https://store.steampowered.com/tags/en/Artificial%20Intelligence/> .

steam:AsymmetricVR a owl:Class, steam:Features ;
  rdfs:label "Asymmetric VR" ;
  rdfs:comment "Asymmetric VR is a feature that involves different experiences for VR and non-VR players in the same game. This can create unique cooperative or competitive scenarios, enhancing the diversity of gameplay." ;
  schema:url <https://store.steampowered.com/tags/en/Asymmetric%20VR/> .

steam:ATV a owl:Class, steam:Features ;
  rdfs:label "ATV" ;
  rdfs:comment "ATV (All-Terrain Vehicle) is a feature that involves the use of off-road vehicles. This can add an element of exploration, racing, or combat to the game, often in rugged, outdoor environments." ;
  rdfs:seeAlso <http://dbpedia.org/resource/All-terrain_vehicle> ;
  schema:url <https://store.steampowered.com/tags/en/ATV/> .

steam:Automation a owl:Class, steam:Features ;
  rdfs:label "Automation" ;
  rdfs:comment "Automation is a feature that allows certain tasks or processes to be automatically controlled or carried out within the game. This can involve resource management, base building, or AI-controlled characters." ;
  rdfs:seeAlso <http://dbpedia.org/resource/Automation> ;
  schema:url <https://store.steampowered.com/tags/en/Automation/> .

steam:BaseBuilding a steam:Features .

steam:Boxing a owl:Class, steam:Features ;
  rdfs:label "Boxing" ;
  rdfs:comment "Boxing, as a feature in games, simulates the sport of boxing, focusing on timing, strategy, and quick reflexes. It often involves one-on-one combat where players control a boxer." ;
  rdfs:seeAlso <http://dbpedia.org/resource/Boxing> ;
  schema:url <https://store.steampowered.com/tags/en/Boxing/> .

steam:Building a steam:Features .

steam:BulletTime a owl:Class, steam:Features ;
  rdfs:label "Bullet Time" ;
  rdfs:comment "Bullet Time is a feature where time slows down, often during combat scenarios. It allows players to see actions such as bullets moving in slow motion, adding a cinematic feel to the gameplay." ;
  rdfs:seeAlso <http://dbpedia.org/resource/Bullet_time> ;
  schema:url <https://store.steampowered.com/tags/en/Bullet%20Time/> .

steam:CharacterCustomization a owl:Class, steam:Features ;
  rdfs:label "Character Customization" ;
  rdfs:comment "Character Customization is a feature that offers detailed control over the visual design and/or abilities of player characters. It allows players to create unique avatars, enhancing immersion and personal connection to the game world." ;
  rdfs:seeAlso <http://dbpedia.org/resource/Character_creation> ;
  schema:url <https://store.steampowered.com/tags/en/Character%20Customization/> .

steam:ChoicesMatter a owl:Class, steam:Features ;
  rdfs:label "Choices Matter" ;
  rdfs:comment "Choices Matter is a feature where the decisions made by the player significantly affect the course of the game's narrative or gameplay. It often leads to multiple endings, enhancing replayability and player agency." ;
  schema:url <https://store.steampowered.com/tags/en/Choices%20Matter/> .

steam:ClassBased a owl:Class, steam:Features ;
  rdfs:label "Class-Based" ;
  rdfs:comment "Class-Based is a feature that involves the use of distinct character classes, each with their own unique abilities, skills, and roles within the game. This can add depth and variety to gameplay, encouraging different playstyles and strategies." ;
  rdfs:seeAlso <http://dbpedia.org/resource/Character_class> ;
  schema:url <https://store.steampowered.com/tags/en/Class-Based/> .

steam:Combat a owl:Class, steam:Features ;
  rdfs:label "Combat" ;
  rdfs:comment "Combat is a feature that involves fighting between characters. This can take many forms, from melee to ranged, magic to technology, and can be a central part of many game genres." ;
  rdfs:seeAlso <http://dbpedia.org/resource/Combat> ;
  schema:url <https://store.steampowered.com/tags/en/Combat/> .

steam:Conversation a owl:Class, steam:Features ;
  rdfs:label "Conversation" ;
  rdfs:comment "Conversation is a feature that involves dialogue between characters. This can be a key part of narrative-driven games, and can also involve elements of choice and consequence." ;
  rdfs:seeAlso <http://dbpedia.org/resource/Conversation> ;
  schema:url <https://store.steampowered.com/tags/en/Conversation/> .

steam:Crafting a owl:Class, steam:Features ;
  rdfs:label "Crafting" ;
  rdfs:comment "Crafting is a feature that allows players to create new items or equipment from resources. This can be a key part of survival games, RPGs, and more, allowing for customization and progression." ;
  rdfs:seeAlso <http://dbpedia.org/resource/Craft> ;
  schema:url <https://store.steampowered.com/tags/en/Crafting/> .

steam:Deckbuilding a owl:Class, steam:Features ;
  rdfs:label "Deckbuilding" ;
  rdfs:comment "Deckbuilding is a feature that involves creating and customizing a deck of cards to use in gameplay. This is a key part of many card games, and can involve strategic decision-making and planning." ;
  rdfs:seeAlso <http://dbpedia.org/resource/Deck-building_game> ;
  schema:url <https://store.steampowered.com/tags/en/Deckbuilding/> .

steam:Driving a owl:Class, steam:Features ;
  rdfs:label "Driving" ;
  rdfs:comment "Driving is a feature that involves controlling a vehicle. This can be a key part of racing games, but can also feature in a wide range of other genres." ;
  rdfs:seeAlso <http://dbpedia.org/resource/Driving> ;
  schema:url <https://store.steampowered.com/tags/en/Driving/> .

steam:Fishing a owl:Class, steam:Features ;
  rdfs:label "Fishing" ;
  rdfs:comment "Fishing is a feature that involves catching fish. This can be a relaxing pastime within a larger game, or the central focus of a fishing game." ;
  rdfs:seeAlso <http://dbpedia.org/resource/Fishing> ;
  schema:url <https://store.steampowered.com/tags/en/Fishing/> .

steam:Flight a steam:Features .

steam:FMV a steam:Features .

steam:GridBasedMovement a owl:Class, steam:Features ;
  rdfs:label "Grid-Based Movement" ;
  rdfs:comment "Grid-Based Movement is a feature that restricts movement to a grid. This can be a key part of many strategy and puzzle games, and can add a layer of tactical decision-making to gameplay." ;
  rdfs:seeAlso <http://dbpedia.org/resource/Grid_plan> ;
  schema:url <https://store.steampowered.com/tags/en/Grid-Based%20Movement/> .

steam:GunCustomization a owl:Class, steam:Features ;
  rdfs:label "Gun Customization" ;
  rdfs:comment "Gun Customization is a feature that allows players to modify and personalize firearms. This can be a key part of many shooter games, allowing for a wide range of playstyles and strategies." ;
  rdfs:seeAlso <http://dbpedia.org/resource/Firearm> ;
  schema:url <https://store.steampowered.com/tags/en/Gun%20Customization/> .

steam:HackAndSlash a steam:Features .

steam:Hacking a steam:Features .

steam:HexGrid a owl:Class, steam:Features ;
  rdfs:label "Hex Grid" ;
  rdfs:comment "Hex Grid is a feature that involves a grid of hexagonal tiles. This can be a key part of many strategy games, and can allow for more complex and varied movement than a square grid." ;
  rdfs:seeAlso <http://dbpedia.org/resource/Hex_map> ;
  schema:url <https://store.steampowered.com/tags/en/Hex%20Grid/> .

steam:Hunting a owl:Class, steam:Features ;
  rdfs:label "Hunting" ;
  rdfs:comment "Hunting is a feature that involves tracking and killing animals. This can be a key part of many survival games, and can involve elements of tracking, stealth, and resource management." ;
  rdfs:seeAlso <http://dbpedia.org/resource/Hunting> ;
  schema:url <https://store.steampowered.com/tags/en/Hunting/> .

steam:InventoryManagement a owl:Class, steam:Features ;
  rdfs:label "Inventory Management" ;
  rdfs:comment "Inventory Management is a feature that involves managing a limited inventory of items. This can be a key part of many RPGs and survival games, and can involve strategic decision-making and planning." ;
  rdfs:seeAlso <http://dbpedia.org/resource/Inventory> ;
  schema:url <https://store.steampowered.com/tags/en/Inventory%20Management/> .

steam:LevelEditor a owl:Class, steam:Features ;
  rdfs:label "Level Editor" ;
  rdfs:comment "Level Editor is a feature that allows players to create and share their own levels or maps. This can add a significant amount of replayability to a game, and allows for a high degree of player creativity." ;
  rdfs:seeAlso <http://dbpedia.org/resource/Level_editor> ;
  schema:url <https://store.steampowered.com/tags/en/Level%20Editor/> .

steam:Linear a owl:Class, steam:Features ;
  rdfs:label "Linear" ;
  rdfs:comment "Linear is a feature that involves a set, predetermined path through the game. This can be a key part of many narrative-driven games, and often involves a strong focus on storytelling." ;
  rdfs:seeAlso <http://dbpedia.org/resource/Linearity> ;
  schema:url <https://store.steampowered.com/tags/en/Linear/> .

steam:MartialArts a owl:Class, steam:Features ;
  rdfs:label "Martial Arts" ;
  rdfs:comment "Martial Arts is a feature that involves combat techniques. This can be a key part of many action and fighting games, and often involves a focus on skill and timing." ;
  rdfs:seeAlso <http://dbpedia.org/resource/Martial_arts> ;
  schema:url <https://store.steampowered.com/tags/en/Martial%20Arts/> .

steam:Mining a steam:Features .

steam:Moddable a owl:Class, steam:Features ;
  rdfs:label "Moddable" ;
  rdfs:comment "Moddable is a feature that allows players to modify the game. This can add a significant amount of replayability to a game, and allows for a high degree of player creativity." ;
  rdfs:seeAlso <http://dbpedia.org/resource/Video_game_modding> ;
  schema:url <https://store.steampowered.com/tags/en/Moddable/> .

steam:MultipleEndings a owl:Class, steam:Features ;
  rdfs:label "Multiple Endings" ;
  rdfs:comment "Multiple Endings is a feature that involves different potential outcomes to the game's story. This can be a key part of many narrative-driven games, and often involves a focus on player choice and branching narratives." ;
  rdfs:seeAlso <http://dbpedia.org/resource/Types_of_fiction_with_multiple_endings> ;
  schema:url <https://store.steampowered.com/tags/en/Multiple%20Endings/> .

steam:MusicBasedProceduralGeneration a owl:Class, steam:Features ;
  rdfs:label "Music-Based Procedural Generation" ;
  rdfs:comment "Music-Based Procedural Generation is a feature that involves generating content based on music. This can be a key part of many rhythm and music games, and often involves a unique and dynamic gameplay experience." ;
  rdfs:seeAlso <http://dbpedia.org/resource/Procedural_generation> ;
  schema:url <https://store.steampowered.com/tags/en/Music-Based%20Procedural%20Generation/> .

steam:Narration a owl:Class, steam:Features ;
  rdfs:label "Narration" ;
  rdfs:comment "Narration is a feature that involves a narrator telling a story. This can be a key part of many narrative-driven games, and often involves a focus on storytelling and atmosphere." ;
  rdfs:seeAlso <http://dbpedia.org/resource/Narration> ;
  schema:url <https://store.steampowered.com/tags/en/Narration/> .

steam:NavalCombat a owl:Class, steam:Features ;
  rdfs:label "Naval Combat" ;
  rdfs:comment "Naval Combat is a feature that involves combat between ships or naval vessels. This can be a key part of many strategy and simulation games, and often involves a focus on tactics and positioning." ;
  rdfs:seeAlso <http://dbpedia.org/resource/Naval_warfare> ;
  schema:url <https://store.steampowered.com/tags/en/Naval%20Combat/> .

steam:Nonlinear a owl:Class, steam:Features ;
  rdfs:label "Nonlinear" ;
  rdfs:comment "Nonlinear is a feature that involves a non-predetermined path through the game. This can be a key part of many open-world and adventure games, and often involves a focus on exploration and player choice." ;
  rdfs:seeAlso <http://dbpedia.org/resource/Nonlinear_gameplay> ;
  schema:url <https://store.steampowered.com/tags/en/Nonlinear/> .

steam:OpenWorld a steam:Features .

steam:PermaDeath a owl:Class, steam:Features ;
  rdfs:label "Perma Death" ;
  rdfs:comment "Perma Death is a feature that involves permanent death for player characters. This can be a key part of many roguelike and survival games, and often involves a high level of challenge and tension." ;
  rdfs:seeAlso <http://dbpedia.org/resource/Permadeath> ;
  schema:url <https://store.steampowered.com/tags/en/Perma%20Death/> .

steam:Physics a owl:Class, steam:Features ;
  rdfs:label "Physics" ;
  rdfs:comment "Physics is a feature that involves the simulation of physical systems. This can be a key part of many simulation and puzzle games, and often involves a focus on realism and interactivity." ;
  rdfs:seeAlso <http://dbpedia.org/resource/Physics_engine> ;
  schema:url <https://store.steampowered.com/tags/en/Physics/> .

steam:ProceduralGeneration a owl:Class, steam:Features ;
  rdfs:label "Procedural Generation" ;
  rdfs:comment "Procedural Generation is a feature that involves generating game content algorithmically rather than manually. This can be a key part of many roguelike and sandbox games, and often involves a high level of replayability." ;
  rdfs:seeAlso <http://dbpedia.org/resource/Procedural_generation> ;
  schema:url <https://store.steampowered.com/tags/en/Procedural%20Generation/> .

steam:PvE a owl:Class, steam:Features ;
  rdfs:label "PvE" ;
  rdfs:comment "PvE (Player versus Environment) is a feature that involves players battling against computer-controlled enemies or challenges. This can be a key part of many role-playing and action games, and often involves a focus on cooperation and teamwork." ;
  rdfs:seeAlso <http://dbpedia.org/resource/Player_versus_environment> ;
  schema:url <https://store.steampowered.com/tags/en/PvE/> .

steam:PvP a owl:Class, steam:Features ;
  rdfs:label "PvP" ;
  rdfs:comment "PvP (Player versus Player) is a feature that involves players battling against each other. This can be a key part of many competitive and multiplayer games, and often involves a focus on skill and competition." ;
  rdfs:seeAlso <http://dbpedia.org/resource/Player_versus_player> ;
  schema:url <https://store.steampowered.com/tags/en/PvP/> .

steam:QuickTimeEvents a owl:Class, steam:Features ;
  rdfs:label "Quick-Time Events" ;
  rdfs:comment "Quick-Time Events is a feature that involves timed inputs during cinematic sequences. This can be a key part of many action and adventure games, and often involves a focus on timing and reflexes." ;
  rdfs:seeAlso <http://dbpedia.org/resource/Quick_time_event> ;
  schema:url <https://store.steampowered.com/tags/en/Quick-Time%20Events/> .

steam:ResourceManagement a owl:Class, steam:Features ;
  rdfs:label "Resource Management" ;
  rdfs:comment "Resource Management is a feature that involves managing resources to achieve goals. This can be a key part of many strategy and simulation games, and often involves a focus on planning and strategy." ;
  schema:url <https://store.steampowered.com/tags/en/Resource%20Management/> .

steam:Sailing a owl:Class, steam:Features ;
  rdfs:label "Sailing" ;
  rdfs:comment "Sailing is a feature that involves the navigation of watercraft. This can be a key part of many adventure and simulation games, and often involves a focus on exploration and strategy." ;
  rdfs:seeAlso <http://dbpedia.org/resource/Sailing_(sport)> ;
  schema:url <https://store.steampowered.com/tags/en/Sailing/> .

steam:ScoreAttack a owl:Class, steam:Features ;
  rdfs:label "Score Attack" ;
  rdfs:comment "Score Attack is a feature that involves trying to achieve the highest score possible. This can be a key part of many arcade and action games, and often involves a focus on skill and competition." ;
  rdfs:seeAlso <http://dbpedia.org/resource/Score_attack> ;
  schema:url <https://store.steampowered.com/tags/en/Score%20Attack/> .

steam:Stealth a steam:Features .

steam:StoryRich a owl:Class, steam:Features ;
  rdfs:label "Story Rich" ;
  rdfs:comment "Story Rich is a feature that involves a strong emphasis on narrative. This can be a key part of many adventure and role-playing games, and often involves a focus on character development and world-building." ;
  rdfs:seeAlso <http://dbpedia.org/resource/Interactive_narrative> ;
  schema:url <https://store.steampowered.com/tags/en/Story%20Rich/> .

steam:Tabletop a steam:Features .

steam:TeamBased a owl:Class, steam:Features ;
  rdfs:label "Team-Based" ;
  rdfs:comment "Team-Based is a feature that involves cooperation with other players to achieve goals. This can be a key part of many multiplayer and competitive games, and often involves a focus on teamwork and communication." ;
  rdfs:seeAlso <http://dbpedia.org/resource/Team_sport> ;
  schema:url <https://store.steampowered.com/tags/en/Team-Based/> .

steam:TextBased a steam:Features .

steam:TimeManipulation a owl:Class, steam:Features ;
  rdfs:label "Time Manipulation" ;
  rdfs:comment "Time Manipulation is a feature that involves the control of time as a gameplay mechanic. This can be a key part of many action and puzzle games, and often involves a focus on strategy and problem-solving." ;
  rdfs:seeAlso <http://dbpedia.org/resource/Time_manipulation> ;
  schema:url <https://store.steampowered.com/tags/en/Time%20Manipulation/> .

steam:Trading a steam:Features .

steam:TurnBasedCombat a owl:Class, steam:Features ;
  rdfs:label "Turn-Based Combat" ;
  rdfs:comment "Turn-Based Combat is a feature that involves combat mechanics where players take turns. This can be a key part of many role-playing and strategy games, and often involves a focus on planning and strategy." ;
  rdfs:seeAlso <http://dbpedia.org/resource/Turn-based_strategy> ;
  schema:url <https://store.steampowered.com/tags/en/Turn-Based%20Combat/> .

steam:TurnBasedTactics a steam:Features .

steam:Tutorial a owl:Class, steam:Features ;
  rdfs:label "Tutorial" ;
  rdfs:comment "Tutorial is a feature that involves guided instructions or lessons to teach players how to play the game. This can be a key part of many games, and often involves a focus on learning and skill development." ;
  rdfs:seeAlso <http://dbpedia.org/resource/Tutorial> ;
  schema:url <https://store.steampowered.com/tags/en/Tutorial/> .

steam:VehicularCombat a owl:Class, steam:Features ;
  rdfs:label "Vehicular Combat" ;
  rdfs:comment "Vehicular Combat is a feature that involves combat mechanics using vehicles. This can be a key part of many action and racing games, and often involves a focus on skill and competition." ;
  rdfs:seeAlso <http://dbpedia.org/resource/Vehicular_combat_game> ;
  schema:url <https://store.steampowered.com/tags/en/Vehicular%20Combat/> .

steam:FemaleProtagonist a owl:Class, steam:Features ;
  rdfs:label "Female Protagonist" ;
  rdfs:comment "Female Protagonist is a feature that involves the main character of the game being female. This can be a key part of many games, and often involves a focus on character development and narrative." ;
  rdfs:seeAlso <http://dbpedia.org/resource/Category:Video_games_featuring_female_protagonists> ;
  schema:url <https://store.steampowered.com/tags/en/Female%20Protagonist/> .

steam:SilentProtagonist a owl:Class, steam:Features ;
  rdfs:label "Silent Protagonist" ;
  rdfs:comment "Silent Protagonist is a feature that involves the main character of the game being silent. This can be a key part of many games, and often involves a focus on narrative and player immersion." ;
  rdfs:seeAlso <http://dbpedia.org/resource/Silent_protagonist> ;
  schema:url <https://store.steampowered.com/tags/en/Silent%20Protagonist/> .

steam:VillainProtagonist a owl:Class, steam:Features ;
  rdfs:label "Villain Protagonist" ;
  rdfs:comment "Villain Protagonist is a feature that involves the main character of the game being a villain. This can be a key part of many games, and often involves a focus on character development and narrative." ;
  rdfs:seeAlso <http://dbpedia.org/resource/Villain_protagonist> ;
  schema:url <https://store.steampowered.com/tags/en/Villain%20Protagonist/> .

steam:Minigames a owl:Class, steam:Features ;
  rdfs:label "Minigames" ;
  rdfs:comment "Minigames is a feature that involves smaller games within the main game. This can be a key part of many games, and often involves a focus on variety and additional content." ;
  rdfs:seeAlso <http://dbpedia.org/resource/Minigame> ;
  schema:url <https://store.steampowered.com/tags/en/Minigames/> .

steam:IntentionallyAwkwardControls a owl:Class, steam:Features ;
  rdfs:label "Intentionally Awkward Controls" ;
  rdfs:comment "Intentionally Awkward Controls is a feature that involves game controls that are deliberately difficult to use. This can be a key part of many comedy and challenge-focused games, and often involves a focus on skill and adaptability." ;
  rdfs:seeAlso <http://dbpedia.org/resource/QWOP> ;
  schema:url <https://store.steampowered.com/tags/en/Intentionally%20Awkward%20Controls/> .

# Players tags

steam:FourPlayerLocal a owl:Class, steam:Players ;
  rdfs:label "4 Player Local" ;
  rdfs:comment "4 Player Local represents games that offer the option for up to four players to play simultaneously on the same device. This feature is often found in party and multiplayer games, fostering cooperation and competition among players." ;
  rdfs:subClassOf steam:LocalMultiplayer ;
  schema:url <https://store.steampowered.com/tags/en/4%20Player%20Local/> .

steam:AsynchronousMultiplayer a owl:Class, steam:Players ;
  rdfs:label "Asynchronous Multiplayer" ;
  rdfs:comment "Asynchronous Multiplayer represents games that offer the option for players to participate without all being active at the same time. This feature is often found in strategy and role-playing games, allowing for thoughtful planning and strategy." ;
  rdfs:subClassOf steam:Multiplayer ;
  schema:url <https://store.steampowered.com/tags/en/Asynchronous%20Multiplayer/> .

steam:Coop a owl:Class, steam:Players ;
  rdfs:label "Co-op" ;
  rdfs:comment "Co-op represents games that offer the option for players to work together cooperatively. This feature is often found in action and role-playing games, promoting teamwork and cooperation among players." ;
  rdfs:subClassOf schema:CoOp ;
  rdfs:seeAlso <http://dbpedia.org/resource/Cooperative_gameplay> ;
  schema:url <https://store.steampowered.com/tags/en/Co-op/> .

steam:CoopCampaign a owl:Class, steam:Players ;
  rdfs:label "Co-op Campaign" ;
  rdfs:comment "Co-op Campaign represents games that offer the option for players to play through the game's campaign or story mode cooperatively. This feature is often found in action and role-playing games, fostering teamwork and shared narrative experiences." ;
  rdfs:subClassOf steam:Coop ;
  schema:url <https://store.steampowered.com/tags/en/Co-op%20Campaign/> .

steam:LocalCoop a owl:Class, steam:Players ;
  rdfs:label "Local Co-Op" ;
  rdfs:comment "Local Co-Op represents games that offer the option for players to play cooperatively on the same device. This feature is often found in action and party games, promoting cooperation and shared experiences." ;
  rdfs:subClassOf steam:Coop ;
  rdfs:seeAlso <http://dbpedia.org/resource/Cooperative_gameplay> ;
  schema:url <https://store.steampowered.com/tags/en/Local%20Co-Op/> .

steam:LocalMultiplayer a owl:Class, steam:Players ;
  rdfs:label "Local Multiplayer" ;
  rdfs:comment "Local Multiplayer represents games that offer the option for multiple players to play on the same device. This feature is often found in party and multiplayer games, fostering competition and shared experiences." ;
  rdfs:subClassOf steam:Multiplayer ;
  schema:url <https://store.steampowered.com/tags/en/Local%20Multiplayer/> .

steam:MassivelyMultiplayer a owl:Class, steam:Players ;
  rdfs:label "Massively Multiplayer" ;
  rdfs:comment "Massively Multiplayer represents games that offer the option to support large numbers of players within the same game world. This feature is often found in online role-playing games, promoting social interaction and cooperation among a large number of players." ;
  rdfs:subClassOf steam:Multiplayer ;
  rdfs:seeAlso <http://dbpedia.org/resource/Massively_multiplayer_online_game> ;
  schema:url <https://store.steampowered.com/tags/en/Massively%20Multiplayer/> .

steam:Multiplayer a owl:Class, steam:Players ;
  rdfs:label "Multiplayer" ;
  rdfs:comment "Multiplayer represents games that offer the option for multiple players to play together. This feature is often found in action and strategy games, fostering competition and cooperation among players." ;
  rdfs:subClassOf schema:MultiPlayer ;
  rdfs:seeAlso <http://dbpedia.org/resource/Multiplayer_video_game> ;
  schema:url <https://store.steampowered.com/tags/en/Multiplayer/> .

steam:OnlineCoop a owl:Class, steam:Players ;
  rdfs:label "Online Co-Op" ;
  rdfs:comment "Online Co-Op represents games that offer the option for players to play cooperatively over the internet. This feature is often found in action and role-playing games, promoting teamwork and social interaction among players." ;
  rdfs:subClassOf steam:Coop ;
  schema:url <https://store.steampowered.com/tags/en/Online%20Co-Op/> .

steam:Singleplayer a owl:Class, steam:Players ;
  rdfs:label "Singleplayer" ;
  rdfs:comment "Singleplayer represents games that offer the option for a single player to play alone. This feature is often found in action, adventure, and role-playing games, fostering narrative and character development." ;
  rdfs:subClassOf schema:SinglePlayer ;
  rdfs:seeAlso <http://dbpedia.org/resource/Single-player_video_game> ;
  schema:url <https://store.steampowered.com/tags/en/Singleplayer/> .

# Other tags

steam:BasedOnANovel a owl:Class, steam:Other ;
  rdfs:label "Based on a Novel" ;
  rdfs:comment "Based on a Novel represents games that are adaptations of literary works. These games often strive to capture the narrative, themes, and characters of the original novels, providing an interactive experience of the story." ;
  rdfs:seeAlso <http://dbpedia.org/resource/Video_game_adaptation> ;
  schema:url <https://store.steampowered.com/tags/en/Based%20On%20A%20Novel/> .

steam:Batman a owl:Class, steam:Other ;
  rdfs:label "Batman" ;
  rdfs:comment "Batman represents games that are based on the Batman franchise. These games often feature Batman as the main character and are set in Gotham City, involving themes of crime-fighting, detective work, and superhero action." ;
  rdfs:seeAlso <http://dbpedia.org/resource/Batman> ;
  schema:url <https://store.steampowered.com/tags/en/Batman/> .

steam:Documentary a owl:Class, steam:Other ;
  rdfs:label "Documentary" ;
  rdfs:comment "Documentary represents media that aim to document reality, providing factual information and often focusing on a particular subject or theme." ;
  rdfs:seeAlso <http://dbpedia.org/resource/Documentary_film> ;
  schema:url <https://store.steampowered.com/tags/en/Documentary/> .

steam:Drama a owl:Class, steam:Other ;
  rdfs:label "Drama" ;
  rdfs:comment "Drama represents media that focus on dramatic, emotional storytelling. These games often involve complex characters, moral dilemmas, and narrative arcs that evoke emotional responses from the players." ;
  rdfs:seeAlso <http://dbpedia.org/resource/Drama> ;
  schema:url <https://store.steampowered.com/tags/en/Drama/> .

steam:DungeonsAndDragons a owl:Class, steam:Other ;
  rdfs:label "Dungeons & Dragons" ;
  rdfs:comment "Dungeons & Dragons represents media that are based on the Dungeons & Dragons franchise." ;
  rdfs:seeAlso <http://dbpedia.org/resource/Dungeons_%26_Dragons> ;
  schema:url <https://store.steampowered.com/tags/en/Dungeons%20%26%20Dragons/> .

steam:Episodic a owl:Class, steam:Other ;
  rdfs:label "Episodic" ;
  rdfs:comment "Episodic represents games that are released in parts or episodes, with each episode often featuring a self-contained story that contributes to a larger narrative. This format allows for ongoing storytelling and character development." ;
  rdfs:seeAlso <http://dbpedia.org/resource/Episodic_video_game> ;
  schema:url <https://store.steampowered.com/tags/en/Episodic/> .

steam:Experience a owl:Class, steam:Other ;
  rdfs:label "Experience" ;
  rdfs:comment "Experience represents games that prioritize creating a unique, immersive experience for the player. These games often focus on atmosphere, aesthetics, and exploration, rather than traditional gameplay mechanics." ;
  schema:url <https://store.steampowered.com/tags/en/Experience/> .

steam:FeatureFilm a owl:Class, steam:Other ;
  rdfs:label "Feature Film" ;
  rdfs:comment "Feature Film represents games that are associated with a feature film. These games often share the same characters, settings, and storylines as the film, providing an interactive extension of the cinematic experience." ;
  rdfs:seeAlso <http://dbpedia.org/resource/Feature_film> ;
  schema:url <https://store.steampowered.com/tags/en/Feature%20Film/> .

steam:GamesWorkshop a owl:Class, steam:Other ;
  rdfs:label "Games Workshop" ;
  rdfs:comment "Games Workshop represents games that are based on franchises created by Games Workshop. These games often feature elements of fantasy or science fiction, including Warhammer 40,000 and Warhammer Fantasy Battles." ;
  rdfs:seeAlso <http://dbpedia.org/resource/Games_Workshop> ;
  schema:url <https://store.steampowered.com/tags/en/Games%20Workshop/> .

steam:Indie a owl:Class, steam:Other ;
  rdfs:label "Indie" ;
  rdfs:comment "Indie represents games that are developed by independent studios. These games often feature innovative gameplay, unique art styles, and personal creative visions, free from the constraints of larger publishers." ;
  rdfs:seeAlso <http://dbpedia.org/resource/Indie_game> ;
  schema:url <https://store.steampowered.com/tags/en/Indie/> .

steam:LaraCroft a owl:Class, steam:Other ;
  rdfs:label "Lara Croft" ;
  rdfs:comment "Lara Croft represents games that feature Lara Croft as the main character. These games are often part of the Tomb Raider franchise, involving themes of adventure, archaeology, and action." ;
  rdfs:seeAlso <http://dbpedia.org/resource/Lara_Croft> ;
  schema:url <https://store.steampowered.com/tags/en/Lara%20Croft/> .

steam:LEGO a owl:Class, steam:Other ;
  rdfs:label "LEGO" ;
  rdfs:comment "LEGO represents games that are based on the LEGO brand. These games often feature LEGO-style graphics, building mechanics, and themes from various LEGO sets and franchises." ;
  rdfs:seeAlso <http://dbpedia.org/resource/Lego> ;
  schema:url <https://store.steampowered.com/tags/en/LEGO/> .

steam:Mod a owl:Class, steam:Other ;
  rdfs:label "Mod" ;
  rdfs:comment "Mod represents games that support or are based on modifications (mods). Mods are player-created content that can alter or add to the original game, often enhancing replayability and community engagement." ;
  rdfs:seeAlso <http://dbpedia.org/resource/Mod_(video_gaming)> ;
  schema:url <https://store.steampowered.com/tags/en/Mod/> .

steam:Movie a owl:Class, steam:Other ;
  rdfs:label "Movie" ;
  rdfs:comment "When games are tagged with movie they often adapted from and share the same characters, settings, and storylines as a movie, providing an interactive extension of the cinematic experience. Alternatively, this may also tag software that is used to play or produce movies." ;
  schema:url <https://store.steampowered.com/tags/en/Movie/> .

steam:Music a owl:Class, steam:Other ;
  rdfs:label "Music" ;
  rdfs:comment "Music represents games that focus on music, either through gameplay mechanics, such as rhythm games, or through a notable musical score. These games often provide a rich auditory experience and may involve musical creativity." ;
  rdfs:seeAlso <http://dbpedia.org/resource/Music_video_game> ;
  schema:url <https://store.steampowered.com/tags/en/Music/> .

steam:RealTime a owl:Class, steam:Other ;
  rdfs:label "Real-Time" ;
  rdfs:comment "Real-Time represents games that occur in real-time, where game events progress continuously according to the game clock. This feature is often found in strategy and simulation games, requiring players to make decisions in the moment." ;
  rdfs:seeAlso <http://dbpedia.org/resource/Turns,_rounds_and_time-keeping_systems_in_games> ;
  schema:url <https://store.steampowered.com/tags/en/Real-Time/> .

steam:RealTimeWithPause a owl:Class, steam:Other ;
  rdfs:label "Real-Time with Pause" ;
  rdfs:comment "Real-Time with Pause represents games that occur in real-time but allow the player to pause the game. This feature is often found in strategy and role-playing games, allowing players to plan actions while the game is paused." ;
  rdfs:seeAlso <http://dbpedia.org/resource/Turns,_rounds_and_time-keeping_systems_in_games> ;
  schema:url <https://store.steampowered.com/tags/en/Real-Time%20with%20Pause/> .

steam:Remake a owl:Class, steam:Other ;
  rdfs:label "Remake" ;
  rdfs:comment "Remake represents games that are remakes of previous games. These games often feature updated graphics, gameplay, and content, while preserving the original game's core experience." ;
  rdfs:seeAlso <http://dbpedia.org/resource/Video_game_remake> ;
  schema:url <https://store.steampowered.com/tags/en/Remake/> .

steam:Sequel a owl:Class, steam:Other ;
  rdfs:label "Sequel" ;
  rdfs:comment "Sequel represents games that are sequels to previous games. These games often continue the story, themes, and gameplay of the original game, while introducing new content and improvements." ;
  rdfs:seeAlso <http://dbpedia.org/resource/Sequel> ;
  schema:url <https://store.steampowered.com/tags/en/Sequel/> .

steam:Soundtrack a owl:Class, steam:Other ;
  rdfs:label "Soundtrack" ;
  rdfs:comment "Soundtrack represents games that are notable for their soundtrack. These games often feature original music that enhances the game's atmosphere, narrative, and emotional impact." ;
  rdfs:seeAlso <http://dbpedia.org/resource/Soundtrack> ;
  schema:url <https://store.steampowered.com/tags/en/Soundtrack/> .

steam:StarWars a owl:Class, steam:Other ;
  rdfs:label "Star Wars" ;
  rdfs:comment "Star Wars represents games that are based on the Star Wars franchise. These games often feature elements of space opera, including epic battles, and themes of good versus evil." ;
  rdfs:seeAlso <http://dbpedia.org/resource/Star_Wars> ;
  schema:url <https://store.steampowered.com/tags/en/Star%20Wars/> .

steam:TimeAttack a owl:Class, steam:Other ;
  rdfs:label "Time Attack" ;
  rdfs:comment "Time Attack represents games that feature a time attack mode, where players aim to complete a level or task in the shortest time possible. This feature is often found in racing and platformer games, promoting speed and skill." ;
  schema:url <https://store.steampowered.com/tags/en/Time%20Attack/> .

steam:TurnBased a owl:Class, steam:Other ;
  rdfs:label "Turn-Based" ;
  rdfs:comment "Turn-Based represents games that are played in turns, where players take turns to perform actions. This feature is often found in strategy and role-playing games, allowing for thoughtful planning and strategy." ;
  schema:url <https://store.steampowered.com/tags/en/Turn-Based/> .

steam:Warhammer40K a owl:Class, steam:Other ;
  rdfs:label "Warhammer 40K" ;
  rdfs:comment "Warhammer 40K represents games that are based on the Warhammer 40,000 franchise. These games often feature elements of science fantasy, including epic battles, complex lore, and a grimdark setting." ;
  rdfs:seeAlso <http://dbpedia.org/resource/Warhammer_40,000> ;
  schema:url <https://store.steampowered.com/tags/en/Warhammer%2040K/> .


